examples/miller/prob/prob_binomialScript.sml
@@ -1,9 +1,9 @@
 open HolKernel Parse boolLib bossLib arithmeticTheory pred_setTheory
      listTheory sequenceTheory state_transformerTheory
-     probabilityTheory HurdUseful extra_numTheory combinTheory
+     old_probabilityTheory hurdUtils extra_numTheory combinTheory
      pairTheory realTheory realLib extra_boolTheory
      extra_pred_setTheory prob_algebraTheory probTheory
-     extra_realTheory extra_pred_setTools measureTheory numTheory
+     extra_realTheory extra_pred_setTools old_measureTheory numTheory
      simpLib seqTheory sequenceTools subtypeTheory res_quanTheory
      binomialTheory sumTheory;
 
