src/probability/probabilityScript.sml
@@ -2,50 +2,45 @@
 (* Probability Theory                                                        *)
 (* Authors: Tarek Mhamdi, Osman Hasan, Sofiene Tahar                         *)
 (* HVG Group, Concordia University, Montreal                                 *)
+(*                                                                           *)
+(* Updated by Chun Tian (2019)                                               *)
+(* Fondazione Bruno Kessler and University of Trento, Italy                  *)
 (* ------------------------------------------------------------------------- *)
 (* Based on the work of Aaron Coble, Cambridge University                    *)
 (* ------------------------------------------------------------------------- *)
 
-(* interactive mode
-app load ["arithmeticTheory", "realTheory", "prim_recTheory", "seqTheory",
-          "pred_setTheory","res_quanTheory", "res_quanTools", "listTheory",
-          "transcTheory", "rich_listTheory", "pairTheory",
-          "combinTheory", "realLib", "optionTheory", "real_sigmaTheory",
-          "util_probTheory", "extrealTheory", "measureTheory", "lebesgueTheory"];
-quietdec := true;
-*)
-
 open HolKernel Parse boolLib bossLib arithmeticTheory realTheory prim_recTheory
-     seqTheory pred_setTheory res_quanTheory res_quanTools listTheory transcTheory
-     rich_listTheory pairTheory combinTheory realLib  optionTheory
-     real_sigmaTheory util_probTheory extrealTheory measureTheory lebesgueTheory;
+     seqTheory pred_setTheory res_quanTheory res_quanTools transcTheory
+     pairTheory combinTheory realLib optionTheory real_sigmaTheory;
+
+open hurdUtils util_probTheory extrealTheory measureTheory borelTheory
+     lebesgueTheory martingaleTheory;
 
 val _ = new_theory "probability";
 
-val REVERSE = Tactical.REVERSE;
+(* "This task would have been a rather hopeless one before the
+    introduction of Lebesgue's theories of measure and integration. ...
+    But if probability theory was to be based on the above analogies, it
+    still was necessary to make the theories of measure and integration
+    independent of the geometric elements which were in the
+    foreground with Lebesgue. ...
 
-val S_TAC = rpt (POP_ASSUM MP_TAC) >> rpt RESQ_STRIP_TAC;
-val Strip = S_TAC;
+    I wish to call attention to those points of the present exposition
+    which are outside the above-mentioned range of ideas familiar to
+    the specialist. They are the following: Probability distributions
+    in infinite-dimensional spaces (Chapter III, 4); differentiation
+    and integration of mathematical expectations with respect to a
+    parameter (Chapter IV, 5); and especially the theory of conditional
+    probabilities and conditional expectations (Chapter V). ..."
 
-fun K_TAC _ = ALL_TAC;
-val KILL_TAC = POP_ASSUM_LIST K_TAC;
-val Know = Q_TAC KNOW_TAC;
-val Suff = Q_TAC SUFF_TAC;
-val POP_ORW = POP_ASSUM (fn thm => ONCE_REWRITE_TAC [thm]);
-
-fun wrap a = [a];
-val Rewr = DISCH_THEN (REWRITE_TAC o wrap);
-val Rewr' = DISCH_THEN (ONCE_REWRITE_TAC o wrap);
-
-
-(*
- interactive mode
-quietdec := false;
-*)
+  -- A. N. Kolmogorov, Foundations of the Theory of Probability [1] *)
 
 (* ------------------------------------------------------------------------- *)
 (* Basic probability theory definitions.                                     *)
 (* ------------------------------------------------------------------------- *)
+
+val _ = type_abbrev ("p_space", ``:'a m_space``);
+val _ = type_abbrev ("events",  ``:'a set set``);
 
 val p_space_def = Define `p_space = m_space`;
 
@@ -54,46 +49,81 @@ val events_def = Define `events = measurable_sets`;
 val prob_def = Define `prob = measure`;
 
 val prob_space_def = Define
-  `prob_space p = measure_space p /\ (measure p (p_space p) = 1)`;
+   `prob_space p = measure_space p /\ (measure p (p_space p) = 1)`;
 
 val indep_def = Define
-  `indep p a b =
-   a IN events p /\ b IN events p /\
-   (prob p (a INTER b) = prob p a * prob p b)`;
+   `indep p a b = a IN events p /\ b IN events p /\
+                 (prob p (a INTER b) = prob p a * prob p b)`;
+
+(* extension of ``indep``: a set of independent events *)
+val indep_events_def = Define (* new *)
+   `indep_events p E (J :num set) =
+      (!n. n IN J ==> (E n) IN events p) /\
+      !N. N SUBSET J /\ N <> {} /\ FINITE N ==>
+         (prob p (BIGINTER (IMAGE E N)) = PI (prob p) (IMAGE E N))`;
+
+(* extension of ``indep``: a set of pairwise independent events *)
+val pairwise_indep_events_def = Define (* new *)
+   `pairwise_indep_events p E (J :num set) =
+      !i j. i IN J /\ j IN J /\ i <> j ==>
+           (prob p ((E i) INTER (E j)) = prob p (E i) * prob p (E j))`;
 
 val indep_families_def = Define `
-    indep_families p q r = !s t. s IN q /\ t IN r ==> indep p s t`;
+    indep_families (p :'a p_space) (q :'a events) (r :'a events) =
+      !s t. s IN q /\ t IN r ==> indep p s t`;
+
+(* "indep_set" is the name used in Isabelle's IndependentFamily.thy *)
+val _ = overload_on ("indep_set", ``indep_families``);
+val indep_set_def = indep_families_def;
+
+val pairwise_indep_sets_def = Define (* new *)
+   `pairwise_indep_sets (p :'a p_space) (A :num -> 'a events) (J :num set) =
+      !i j. i IN J /\ j IN J /\ i <> j ==> indep_set p (A i) (A j)`;
+
+(* from Isabelle's IndependentFamily.thy (`Pi` in Isabelle/HOL = `DFUNSET` in HOL4) *)
+val indep_sets_def = Define
+   `indep_sets (p :'a p_space) (A :num -> 'a events) (J :num set) =
+     (!n. n IN J ==> (A n) SUBSET events p) /\
+     !N. N SUBSET J /\ N <> {} /\ FINITE N ==>
+         !E. E IN (J --> A) ==> (prob p (BIGINTER (IMAGE E N)) = PI (prob p) (IMAGE E N))`;
 
 val indep_function_def = Define `
     indep_function p =
-   {f |
-    indep_families p (IMAGE (PREIMAGE (FST o f)) UNIV)
-    (IMAGE (PREIMAGE (SND o f)) (events p))}`;
+      {f | indep_families p (IMAGE (PREIMAGE (FST o f)) UNIV)
+                            (IMAGE (PREIMAGE (SND o f)) (events p))}`;
 
-val probably_def = Define `probably p e = (e IN events p) /\ (prob p e = 1)`;
+val probably_def = Define
+   `probably p e = e IN events p /\ (prob p e = 1)`;
 
-val possibly_def = Define `possibly p e = (e IN events p) /\ ~(prob p e = 0)`;
+val possibly_def = Define
+   `possibly p e = e IN events p /\ prob p e <> 0`;
 
+(* this is an abstract random variable *)
 val random_variable_def = Define
    `random_variable X p s = prob_space p /\ X IN measurable (p_space p, events p) s`;
 
+(* is `X x <> NegInf /\ X x <> PosInf` necessary? *)
 val real_random_variable_def = Define
-   `real_random_variable X p = prob_space p /\
-                              (!x. x IN p_space p ==> X x <> NegInf /\ X x <> PosInf) /\
-                              X IN measurable (p_space p, events p) Borel`;
+   `real_random_variable X p =
+      prob_space p /\ (!x. x IN p_space p ==> X x <> NegInf /\ X x <> PosInf) /\
+      X IN measurable (p_space p, events p) Borel`;
 
 val distribution_def = Define
-   `distribution p X = (\s. prob p ((PREIMAGE X s) INTER (p_space p)))`;
+   `distribution (p :'a p_space) X = (\s. prob p ((PREIMAGE X s) INTER p_space p))`;
 
 val joint_distribution_def = Define
-   `joint_distribution p X Y = (\a. prob p (PREIMAGE (\x. (X x, Y x)) a INTER p_space p))`;
+   `joint_distribution (p :'a p_space) X Y =
+      (\a. prob p (PREIMAGE (\x. (X x, Y x)) a INTER p_space p))`;
 
 val joint_distribution3_def = Define
-   `joint_distribution3 p X Y Z = (\a. prob p (PREIMAGE (\x. (X x,Y x, Z x)) a INTER p_space p))`;
+   `joint_distribution3 (p :'a p_space) X Y Z =
+      (\a. prob p (PREIMAGE (\x. (X x,Y x,Z x)) a INTER p_space p))`;
 
 val conditional_distribution_def = Define
-   `conditional_distribution p X Y a b = joint_distribution p X Y (a CROSS b) / distribution p Y b `;
+   `conditional_distribution (p :'a p_space) X Y a b =
+      joint_distribution p X Y (a CROSS b) / distribution p Y b`;
 
+(* expection is just (Lebesgue) integral *)
 val expectation_def = Define
    `expectation = integral`;
 
@@ -101,21 +131,68 @@ val conditional_expectation_def = Define
    `conditional_expectation p X s =
         @f. real_random_variable f p /\
             !g. g IN s ==>
-                (integral p (\x. f x * indicator_fn g x) =
-                 integral p (\x. X x * indicator_fn g x))`;
+                (expectation p (\x. f x * indicator_fn g x) =
+                 expectation p (\x. X x * indicator_fn g x))`;
 
 val conditional_prob_def = Define
-   `conditional_prob p e1 e2 = conditional_expectation p (indicator_fn e1) e2`;
+   `conditional_prob p e1 e2 =
+    conditional_expectation p (indicator_fn e1) e2`;
 
 val rv_conditional_expectation_def = Define
-   `rv_conditional_expectation p s X Y =
-        conditional_expectation p X (IMAGE (\a. (PREIMAGE Y a) INTER p_space p) (subsets s))`;
+   `rv_conditional_expectation (p :'a p_space) s X Y =
+       conditional_expectation p X (IMAGE (\a. (PREIMAGE Y a) INTER p_space p) (subsets s))`;
 
-val indep_rv_def = Define `indep_rv p X Y s t = !A B. (A IN subsets s) /\ (B IN subsets t)
-    ==> indep p (PREIMAGE X A) (PREIMAGE Y B)`;
+(* NOTE: X and Y are forced to have the same types;
+         Added `INTER p_space p` after taking the PREIMAGE. *)
+val indep_rv_def = Define
+   `indep_rv (p :'a p_space) (X :'a -> 'b) (Y :'a -> 'b) s t =
+      !A B. (A IN subsets s) /\ (B IN subsets t) ==>
+            indep p ((PREIMAGE X A) INTER p_space p)
+                    ((PREIMAGE Y B) INTER p_space p)`;
 
+val _ = overload_on ("indep_var", ``indep_rv``); (* the name used in Isabelle/HOL *)
+val indep_var_def = indep_rv_def;
+
+(* Total independence of a set of random variables.
+
+   NOTE: in Isabelle's definition of `indep_vars`, the resulting pre-images
+   from (E n) are further enlarged by their smallest sigma-algebra, i.e.
+
+    `subsets (sigma (p_space) ((PREIMAGE (X n) (E n)) INTER p_space p))`
+
+   This is not necessary (and counter-intuition) but can be proved later as an
+   equivalent definition. And the proof of Kolmogorov's 0-1 law will be slightly
+   more complicated under the current definition.
+   
+   -- Chun Tian, January 31, 2019.
+ *)
+val indep_vars_def = Define (* new *)
+   `indep_vars p X A (J :num set) =
+      (!n. n IN J ==> random_variable (X n) p (A n)) /\
+      !E. E IN (J --> (subsets o A)) ==>
+          indep_events p (\n. (PREIMAGE (X n) (E n)) INTER p_space p) J`;
+
+(* Pairwise independence of a set of random variables *)
+val pairwise_indep_vars_def = Define (* new *)
+   `pairwise_indep_vars p X E (J :num set) =
+      (!n. n IN J ==> random_variable (X n) p (E n)) /\
+      !i j. i IN J /\ j IN J /\ i <> j ==> indep_var p (X i) (X j) (E i) (E j)`;
+
+val indep_real_var_def = Define (* new *)
+   `indep_real_var p X Y (J :num set) =
+      real_random_variable X p /\ real_random_variable Y p /\
+      indep_var p X Y Borel Borel`;
+
+(* total independence of real random variables *)
+val indep_real_vars_def = Define (* new *)
+   `indep_real_vars p X (J :num set) =
+      (!n. n IN J ==> real_random_variable (X n) p) /\
+      indep_vars p X (\n. Borel) J`;
+
+(* this only works in discrete probability spaces *)
 val uniform_distribution_def = Define
-   `uniform_distribution p X s = (\a. (&CARD a / &CARD (space s)):real)`;
+   `uniform_distribution (s :'a algebra) =
+      (\(a :'a set). (&CARD a / &CARD (space s)):extreal)`;
 
 (* ------------------------------------------------------------------------- *)
 (* Basic probability theorems, leading to:                                   *)
@@ -123,17 +200,20 @@ val uniform_distribution_def = Define
 (* ------------------------------------------------------------------------- *)
 
 val POSITIVE_PROB = store_thm
-  ("POSITIVE_PROB", ``!p. positive p = (prob p {} = 0) /\ !s. s IN events p
-         ==> 0 <= prob p s``,
+  ("POSITIVE_PROB",
+  ``!p. positive p = (prob p {} = 0) /\ !s. s IN events p ==> 0 <= prob p s``,
    RW_TAC std_ss [positive_def, prob_def, events_def]);
 
 val INCREASING_PROB = store_thm
-  ("INCREASING_PROB", ``!p. increasing p = !s t. s IN events p /\ t IN events p /\ s SUBSET t
-         ==> prob p s <= prob p t``,
+  ("INCREASING_PROB",
+  ``!p. increasing p = !s t. s IN events p /\ t IN events p /\ s SUBSET t
+        ==> prob p s <= prob p t``,
    RW_TAC std_ss [increasing_def, prob_def, events_def]);
 
 val ADDITIVE_PROB = store_thm
-  ("ADDITIVE_PROB", ``!p. additive p = !s t. s IN events p /\ t IN events p /\ DISJOINT s t
+  ("ADDITIVE_PROB",
+  ``!p. additive p =
+        !s t. s IN events p /\ t IN events p /\ DISJOINT s t /\ s UNION t IN events p
          ==> (prob p (s UNION t) = prob p s + prob p t)``,
    RW_TAC std_ss [additive_def, prob_def, events_def]);
 
@@ -141,14 +221,15 @@ val COUNTABLY_ADDITIVE_PROB = store_thm
   ("COUNTABLY_ADDITIVE_PROB", ``!p. countably_additive p =
        !f. f IN (UNIV -> events p) /\ (!m n. ~(m = n) ==> DISJOINT (f m) (f n)) /\
            BIGUNION (IMAGE f UNIV) IN events p ==>
-          prob p o f sums (prob p (BIGUNION (IMAGE f UNIV)))``,
+         (prob p (BIGUNION (IMAGE f UNIV)) = suminf (prob p o f))``,
    RW_TAC std_ss [countably_additive_def, prob_def, events_def]);
 
 val PROB_SPACE = store_thm
- ("PROB_SPACE", ``!p. prob_space p = sigma_algebra (p_space p, events p) /\ positive p /\
-                 countably_additive p /\ (prob p (p_space p) = 1)``,
-   RW_TAC std_ss [prob_space_def, prob_def, events_def, measure_space_def, p_space_def]
-   >> PROVE_TAC []);
+  ("PROB_SPACE",
+  ``!p. prob_space p = sigma_algebra (p_space p, events p) /\ positive p /\
+                       countably_additive p /\ (prob p (p_space p) = 1)``,
+    RW_TAC std_ss [prob_space_def, prob_def, events_def, measure_space_def, p_space_def]
+ >> PROVE_TAC []);
 
 val EVENTS_SIGMA_ALGEBRA = store_thm
   ("EVENTS_SIGMA_ALGEBRA",
@@ -182,9 +263,12 @@ val PROB_SPACE_COUNTABLY_ADDITIVE = store_thm
 
 val PROB_SPACE_ADDITIVE = store_thm
   ("PROB_SPACE_ADDITIVE",
-   ``!p. prob_space p ==> additive p``,
-   PROVE_TAC [PROB_SPACE_COUNTABLY_ADDITIVE, COUNTABLY_ADDITIVE_ADDITIVE,
-              PROB_SPACE_POSITIVE, EVENTS_ALGEBRA, events_def, p_space_def]);
+  ``!p. prob_space p ==> additive p``,
+    rpt STRIP_TAC
+ >> MATCH_MP_TAC (REWRITE_RULE [premeasure_def] ALGEBRA_PREMEASURE_ADDITIVE)
+ >> IMP_RES_TAC EVENTS_ALGEBRA
+ >> fs [events_def, p_space_def]
+ >> PROVE_TAC [PROB_SPACE_COUNTABLY_ADDITIVE, PROB_SPACE_POSITIVE]);
 
 val PROB_SPACE_INCREASING = store_thm
   ("PROB_SPACE_INCREASING",
@@ -210,7 +294,12 @@ val PROB_ADDITIVE = store_thm
        prob_space p /\ s IN events p /\ t IN events p /\
        DISJOINT s t /\ (u = s UNION t) ==>
        (prob p u = prob p s + prob p t)``,
-   PROVE_TAC [ADDITIVE_PROB, PROB_SPACE_ADDITIVE]);
+    rpt STRIP_TAC
+ >> IMP_RES_TAC PROB_SPACE_ADDITIVE >> art []
+ >> POP_ASSUM (MATCH_MP_TAC o (REWRITE_RULE [ADDITIVE_PROB]))
+ >> art []
+ >> IMP_RES_TAC EVENTS_ALGEBRA
+ >> PROVE_TAC [ALGEBRA_UNION, subsets_def]);
 
 val PROB_COUNTABLY_ADDITIVE = store_thm
   ("PROB_COUNTABLY_ADDITIVE",
@@ -218,7 +307,7 @@ val PROB_COUNTABLY_ADDITIVE = store_thm
        prob_space p /\ f IN (UNIV -> events p) /\
        (!m n. ~(m = n) ==> DISJOINT (f m) (f n)) /\
        (s = BIGUNION (IMAGE f UNIV)) ==>
-       prob p o f sums (prob p s)``,
+       (prob p s = suminf (prob p o f))``,
    RW_TAC std_ss []
    >> Suff `BIGUNION (IMAGE f UNIV) IN events p`
    >- PROVE_TAC [COUNTABLY_ADDITIVE_PROB, PROB_SPACE_COUNTABLY_ADDITIVE]
@@ -226,10 +315,22 @@ val PROB_COUNTABLY_ADDITIVE = store_thm
         Q.SPECL [`(p_space p, events p)`,`f`]) SIGMA_ALGEBRA_ENUM
    >> PROVE_TAC [EVENTS_SIGMA_ALGEBRA]);
 
+val PROB_FINITE = store_thm
+  ("PROB_FINITE",
+  ``!p s. prob_space p /\ s IN events p ==> (prob p s <> NegInf /\ prob p s <> PosInf)``,
+    RW_TAC std_ss [prob_space_def,prob_def,events_def,positive_not_infty,MEASURE_SPACE_POSITIVE]
+ >> RW_TAC std_ss [GSYM le_infty,GSYM extreal_lt_def]
+ >> MATCH_MP_TAC let_trans
+ >> Q.EXISTS_TAC `measure p (p_space p)`
+ >> Reverse (RW_TAC std_ss [])
+ >- METIS_TAC [num_not_infty,lt_infty]
+ >> METIS_TAC [MEASURE_SPACE_SUBSET_MSPACE,INCREASING,MEASURE_SPACE_INCREASING,
+               MEASURE_SPACE_MSPACE_MEASURABLE,p_space_def]);
+
 val PROB_COMPL = store_thm
  ("PROB_COMPL", ``!p s. prob_space p /\ s IN events p
        ==> (prob p (p_space p DIFF s) = 1 - prob p s)``,
-  METIS_TAC [MEASURE_COMPL,prob_space_def,events_def,prob_def,p_space_def]);
+  METIS_TAC [MEASURE_SPACE_FINITE_DIFF,PROB_FINITE,prob_space_def,events_def,prob_def,p_space_def]);
 
 val PROB_INDEP = store_thm
 ("PROB_INDEP", ``!p s t u. indep p s t /\ (u = s INTER t)
@@ -280,18 +381,17 @@ val EVENTS_UNION = store_thm
 
 val INDEP_EMPTY = store_thm
 ("INDEP_EMPTY", ``!p s. prob_space p /\ s IN events p ==> indep p {} s``,
-  RW_TAC real_ss [indep_def, EVENTS_EMPTY, PROB_EMPTY, INTER_EMPTY]);
+  RW_TAC std_ss [indep_def, EVENTS_EMPTY, PROB_EMPTY, INTER_EMPTY,mul_lzero]);
 
 val INTER_PSPACE = store_thm
-("INTER_PSPACE", ``!p s. prob_space p /\ s IN events p
-                   ==> (p_space p INTER s = s)``,
+("INTER_PSPACE", ``!p s. prob_space p /\ s IN events p ==> (p_space p INTER s = s)``,
   RW_TAC std_ss [PROB_SPACE, SIGMA_ALGEBRA, space_def, subsets_def, subset_class_def, SUBSET_DEF]
   >> RW_TAC std_ss [Once EXTENSION, IN_INTER]
   >> PROVE_TAC []);
 
 val INDEP_SPACE = store_thm
 ("INDEP_SPACE", ``!p s. prob_space p /\ s IN events p ==> indep p (p_space p) s``,
-  RW_TAC real_ss [indep_def, EVENTS_SPACE, PROB_UNIV, INTER_PSPACE]);
+  RW_TAC std_ss [indep_def, EVENTS_SPACE, PROB_UNIV, INTER_PSPACE,mul_lone]);
 
 val EVENTS_DIFF = store_thm
 ("EVENTS_DIFF", ``!p s t. prob_space p /\ s IN events p /\ t IN events p
@@ -326,14 +426,14 @@ val PROB_ZERO_UNION = store_thm
       >> RW_TAC std_ss [])
   >> STRIP_TAC
   >> Know `prob p (t DIFF s) = 0`
-  >- (ONCE_REWRITE_TAC [GSYM REAL_LE_ANTISYM]
-      >> REVERSE CONJ_TAC >- PROVE_TAC [PROB_POSITIVE]
+  >- (ONCE_REWRITE_TAC [GSYM le_antisym]
+      >> Reverse CONJ_TAC >- PROVE_TAC [PROB_POSITIVE]
       >> Q.PAT_X_ASSUM `prob p t = 0` (ONCE_REWRITE_TAC o wrap o SYM)
       >> MATCH_MP_TAC PROB_INCREASING
       >> RW_TAC std_ss [DIFF_SUBSET])
   >> STRIP_TAC
   >> Suff `prob p (s UNION t) = prob p s + prob p (t DIFF s)`
-  >- RW_TAC real_ss []
+  >- RW_TAC real_ss [add_rzero]
   >> MATCH_MP_TAC PROB_ADDITIVE
   >> RW_TAC std_ss [DISJOINT_DEF, DIFF_DEF, EXTENSION, IN_UNION, IN_DIFF, NOT_IN_EMPTY, IN_INTER]
   >> PROVE_TAC []);
@@ -346,6 +446,9 @@ val PROB_EQ_COMPL = store_thm
   >> Know `1 - prob p s = 1 - prob p t`
   >- (POP_ASSUM MP_TAC
       >> RW_TAC std_ss [PROB_COMPL])
+  >> `?r1 r2. (prob p t = Normal r1) /\ (prob p s = Normal r2)`
+    by METIS_TAC [extreal_cases,PROB_FINITE]
+  >> FULL_SIMP_TAC std_ss [extreal_of_num_def,extreal_sub_def,extreal_11]
   >> REAL_ARITH_TAC);
 
 val PROB_ONE_INTER = store_thm
@@ -360,7 +463,7 @@ val PROB_ONE_INTER = store_thm
   >> RW_TAC std_ss [] >> POP_ASSUM (K ALL_TAC)
   >> MATCH_MP_TAC PROB_ZERO_UNION
   >> RW_TAC std_ss [PROB_COMPL, EVENTS_COMPL]
-  >> RW_TAC real_ss []);
+  >> RW_TAC real_ss [extreal_of_num_def,extreal_sub_def]);
 
 val EVENTS_COUNTABLE_INTER = store_thm
 ("EVENTS_COUNTABLE_INTER",
@@ -379,8 +482,7 @@ val EVENTS_COUNTABLE_INTER = store_thm
   >> Rewr'
   >> MATCH_MP_TAC EVENTS_COMPL
   >> Know `p_space p DIFF BIGINTER c = BIGUNION (IMAGE (\s. p_space p DIFF s) c)`
-  >- (ONCE_REWRITE_TAC [EXTENSION]
-      >> RW_TAC std_ss [IN_DIFF, IN_BIGUNION, IN_IMAGE, IN_BIGINTER]
+  >- (ONCE_REWRITE_TAC [EXTENSION] >> RW_TAC std_ss [IN_DIFF, IN_BIGUNION, IN_IMAGE, IN_BIGINTER]
       >> EQ_TAC
       >- (RW_TAC std_ss [] >> Q.EXISTS_TAC `p_space p DIFF P`
           >> RW_TAC std_ss [IN_DIFF] >> Q.EXISTS_TAC `P`
@@ -398,19 +500,19 @@ val EVENTS_COUNTABLE_INTER = store_thm
 val ABS_PROB = store_thm
 ("ABS_PROB", ``!p s. prob_space p /\ s IN events p
                 ==> (abs (prob p s) = prob p s)``,
-  RW_TAC std_ss [PROB_POSITIVE,ABS_REFL]);
-
+  RW_TAC std_ss [extreal_abs_def]
+  >> PROVE_TAC [PROB_POSITIVE,abs_refl]);
 
 val PROB_COMPL_LE1 = store_thm
 ("PROB_COMPL_LE1", ``!p s r. prob_space p /\ s IN events p
                       ==> (prob p (p_space p DIFF s) <= r = 1 - r <= prob p s)``,
   RW_TAC std_ss [PROB_COMPL]
-  >> REAL_ARITH_TAC);
+  >> METIS_TAC [sub_le_switch2,PROB_FINITE,num_not_infty]);
 
 val PROB_LE_1 = store_thm
 ("PROB_LE_1", ``!p s. prob_space p /\ s IN events p ==> prob p s <= 1``,
   RW_TAC std_ss []
-  >> Suff `0 <= 1 - prob p s` >- REAL_ARITH_TAC
+  >> Suff `0 <= 1 - prob p s` >- METIS_TAC [sub_zero_le,PROB_FINITE]
   >> RW_TAC std_ss [GSYM PROB_COMPL]
   >> RW_TAC std_ss [EVENTS_COMPL, PROB_POSITIVE]);
 
@@ -421,9 +523,12 @@ val PROB_EQ_BIGUNION_IMAGE = store_thm
        (!m n. ~(m = n) ==> DISJOINT (g m) (g n)) /\
        (!n: num. prob p (f n) = prob p (g n)) ==>
        (prob p (BIGUNION (IMAGE f UNIV)) = prob p (BIGUNION (IMAGE g UNIV)))``,
-  RW_TAC std_ss []
-  >> METIS_TAC [o_DEF,PROB_COUNTABLY_ADDITIVE,SEQ_UNIQ,sums]);
-
+   RW_TAC std_ss []
+   >> Know `prob p (BIGUNION (IMAGE f UNIV)) = suminf (prob p o f)`
+   >- PROVE_TAC [PROB_COUNTABLY_ADDITIVE]
+   >> Know `prob p (BIGUNION (IMAGE g UNIV)) = suminf (prob p o g)`
+   >- PROVE_TAC [PROB_COUNTABLY_ADDITIVE]
+   >> METIS_TAC [o_DEF]);
 
 val PROB_FINITELY_ADDITIVE = store_thm
   ("PROB_FINITELY_ADDITIVE",
@@ -431,61 +536,59 @@ val PROB_FINITELY_ADDITIVE = store_thm
        prob_space p /\ f IN ((count n) -> events p) /\
        (!a b. a < n /\ b < n /\ ~(a = b) ==> DISJOINT (f a) (f b)) /\
        (s = BIGUNION (IMAGE f (count n))) ==>
-       (sum (0, n) (prob p o f) = prob p s)``,
-   RW_TAC std_ss [IN_FUNSET, IN_COUNT]
-   >> Suff
-      `(prob p o (\m. if m < n then f m else {})) sums
-       prob p (BIGUNION (IMAGE f (count n))) /\
-       (prob p o (\m. if m < n then f m else {})) sums
-       sum (0, n) (prob p o f)`
-   >- PROVE_TAC [SUM_UNIQ]
-   >> REVERSE CONJ_TAC
-   >- (Know
-       `sum (0,n) (prob p o f) =
-        sum (0,n) (prob p o (\m. (if m < n then f m else {})))`
-       >- (MATCH_MP_TAC SUM_EQ
-           >> RW_TAC arith_ss [o_THM])
-       >> Rewr
-       >> MATCH_MP_TAC SER_0
-       >> RW_TAC arith_ss [o_THM, PROB_EMPTY])
-   >> Know
-      `BIGUNION (IMAGE f (count n)) =
-       BIGUNION (IMAGE (\m. (if m < n then f m else {})) UNIV)`
-   >- (RW_TAC std_ss [EXTENSION,IN_BIGUNION_IMAGE, IN_COUNT, IN_UNIV]
-       >> PROVE_TAC [NOT_IN_EMPTY])
-   >> Rewr
-   >> MATCH_MP_TAC PROB_COUNTABLY_ADDITIVE
-   >> BasicProvers.NORM_TAC std_ss
-      [IN_FUNSET, IN_UNIV, DISJOINT_EMPTY, EVENTS_EMPTY]);
+        (prob p s = SIGMA (prob p o f) (count n))``,
+  RW_TAC std_ss [IN_FUNSET, IN_COUNT]
+  >> Suff `(ext_suminf (prob p o (\m. if m < n then f m else {})) = prob p (BIGUNION (IMAGE f (count n)))) /\
+           (ext_suminf (prob p o (\m. if m < n then f m else {})) = SIGMA (prob p o f) (count n))`
+  >- METIS_TAC []
+  >> Reverse CONJ_TAC
+  >- (Know `SIGMA (prob p o f) (count n) = SIGMA (prob p o (\m. (if m < n then f m else {}))) (count n)`
+      >- ((MATCH_MP_TAC o REWRITE_RULE [FINITE_COUNT] o Q.ISPEC `count n`) EXTREAL_SUM_IMAGE_EQ
+          >> RW_TAC std_ss [IN_COUNT]
+          >> METIS_TAC [PROB_FINITE])
+      >> RW_TAC std_ss []
+      >> MATCH_MP_TAC ext_suminf_sum
+      >> RW_TAC std_ss [PROB_EMPTY,PROB_POSITIVE,le_refl]
+      >> METIS_TAC [NOT_LESS])
+  >> Know `BIGUNION (IMAGE f (count n)) = BIGUNION (IMAGE (\m. (if m < n then f m else {})) UNIV)`
+  >- (RW_TAC std_ss [EXTENSION,IN_BIGUNION_IMAGE, IN_COUNT, IN_UNIV]
+      >> METIS_TAC [NOT_IN_EMPTY])
+  >> Rewr
+  >> MATCH_MP_TAC (GSYM PROB_COUNTABLY_ADDITIVE)
+  >> RW_TAC std_ss [IN_FUNSET, IN_UNIV, DISJOINT_EMPTY]
+  >> METIS_TAC [EVENTS_EMPTY]);
 
 val ABS_1_MINUS_PROB = store_thm
   ("ABS_1_MINUS_PROB",
-   ``!p s.
-       prob_space p /\ s IN events p /\ ~(prob p s = 0) ==>
-       abs (1 - prob p s) < 1``,
-   RW_TAC std_ss []
-   >> Know `0 <= prob p s` >- PROVE_TAC [PROB_POSITIVE]
-   >> Know `prob p s <= 1` >- PROVE_TAC [PROB_LE_1]
-   >> RW_TAC std_ss [abs]
-   >> REPEAT (POP_ASSUM MP_TAC)
-   >> REAL_ARITH_TAC);
+  ``!p s.
+      prob_space p /\ s IN events p /\ ~(prob p s = 0) ==>
+      abs (1 - prob p s) < 1``,
+  RW_TAC std_ss []
+  >> Know `0 <= prob p s` >- PROVE_TAC [PROB_POSITIVE]
+  >> Know `prob p s <= 1` >- PROVE_TAC [PROB_LE_1]
+  >> `?r. prob p s = Normal r` by METIS_TAC [PROB_FINITE,extreal_cases]
+  >> FULL_SIMP_TAC std_ss [extreal_of_num_def,extreal_sub_def,extreal_abs_def,
+                           extreal_lt_eq,extreal_le_def,extreal_11]
+  >> RW_TAC std_ss [abs]
+  >> REPEAT (POP_ASSUM MP_TAC)
+  >> REAL_ARITH_TAC);
 
 val PROB_INCREASING_UNION = store_thm
   ("PROB_INCREASING_UNION",
-   ``!p s f.
-       prob_space p /\ f IN (UNIV -> events p) /\
-       (!n. f n SUBSET f (SUC n)) /\ (s = BIGUNION (IMAGE f UNIV)) ==>
-       prob p o f --> prob p s``,
+   ``!p f.
+       prob_space p /\ f IN (UNIV -> events p) /\ (!n. f n SUBSET f (SUC n)) ==>
+       (sup (IMAGE (prob p o f) UNIV) = prob p (BIGUNION (IMAGE f UNIV)))``,
    RW_TAC std_ss [prob_space_def, events_def, prob_def, MONOTONE_CONVERGENCE]);
 
 val PROB_SUBADDITIVE = store_thm
   ("PROB_SUBADDITIVE",
-   ``!p s t u.
-       prob_space p /\ t IN events p /\ u IN events p /\ (s = t UNION u) ==>
-       prob p s <= prob p t + prob p u``,
+   ``!p t u.
+       prob_space p /\ t IN events p /\ u IN events p ==>
+       prob p (t UNION u) <= prob p t + prob p u``,
    RW_TAC std_ss []
    >> Know `t UNION u = t UNION (u DIFF t)`
-   >- (RW_TAC std_ss [EXTENSION, IN_UNION, IN_DIFF]
+   >- (SET_EQ_TAC
+       >> RW_TAC std_ss [IN_UNION, IN_DIFF]
        >> PROVE_TAC [])
    >> Rewr
    >> Know `u DIFF t IN events p`
@@ -495,61 +598,53 @@ val PROB_SUBADDITIVE = store_thm
    >- (MATCH_MP_TAC PROB_ADDITIVE
        >> RW_TAC std_ss [DISJOINT_ALT, IN_DIFF])
    >> Rewr
-   >> MATCH_MP_TAC REAL_LE_LADD_IMP
+   >> MATCH_MP_TAC le_ladd_imp
    >> MATCH_MP_TAC PROB_INCREASING
    >> RW_TAC std_ss [DIFF_DEF, SUBSET_DEF, GSPECIFICATION]);
 
 val PROB_COUNTABLY_SUBADDITIVE = store_thm
   ("PROB_COUNTABLY_SUBADDITIVE",
    ``!p f.
-       prob_space p /\ (IMAGE f UNIV) SUBSET events p /\
-       summable (prob p o f) ==>
+       prob_space p /\ (IMAGE f UNIV) SUBSET events p ==>
        prob p (BIGUNION (IMAGE f UNIV)) <= suminf (prob p o f)``,
-   RW_TAC std_ss [SUBSET_DEF, IN_IMAGE, IN_UNIV]
-   >> Know `(prob p o f) sums suminf (prob p o f)`
-   >- PROVE_TAC [SUMMABLE_SUM]
-   >> RW_TAC std_ss [sums]
-   >> Know
-      `prob p o (\n. BIGUNION (IMAGE f (count n))) -->
-       prob p (BIGUNION (IMAGE f UNIV))`
-   >- (MATCH_MP_TAC PROB_INCREASING_UNION
-       >> RW_TAC std_ss [IN_FUNSET, IN_UNIV] >|
-       [MATCH_MP_TAC EVENTS_COUNTABLE_UNION
-        >> RW_TAC std_ss [SUBSET_DEF, IN_IMAGE, image_countable,
-                          COUNTABLE_COUNT]
-        >> PROVE_TAC [],
-        RW_TAC std_ss [SUBSET_DEF, IN_BIGUNION, IN_IMAGE, IN_COUNT]
-        >> PROVE_TAC [LT_SUC],
-        RW_TAC std_ss [EXTENSION, IN_BIGUNION_IMAGE, IN_UNIV, IN_COUNT]
-        >> REVERSE EQ_TAC >- PROVE_TAC []
-        >> RW_TAC std_ss []
-        >> Q.EXISTS_TAC `SUC x'`
-        >> Q.EXISTS_TAC `x'`
-        >> RW_TAC arith_ss []])
-   >> STRIP_TAC
-   >> MATCH_MP_TAC SEQ_LE
-   >> Q.EXISTS_TAC `prob p o (\n. BIGUNION (IMAGE f (count n)))`
-   >> Q.EXISTS_TAC `(\n. sum (0,n) (prob p o f))`
-   >> RW_TAC std_ss []
-   >> Q.EXISTS_TAC `0`
-   >> RW_TAC arith_ss [o_THM]
-   >> Induct_on `n`
-   >- RW_TAC std_ss [o_THM, COUNT_ZERO, IMAGE_EMPTY, BIGUNION_EMPTY, PROB_EMPTY,
-                     sum, REAL_LE_REFL]
-   >> RW_TAC std_ss [o_THM, COUNT_SUC, IMAGE_INSERT, BIGUNION_INSERT, sum]
-   >> ONCE_REWRITE_TAC [REAL_ADD_SYM]
-   >> RW_TAC arith_ss []
-   >> Suff
-      `prob p (f n UNION BIGUNION (IMAGE f (count n))) <=
-       prob p (f n) + prob p (BIGUNION (IMAGE f (count n)))`
-   >- (POP_ASSUM MP_TAC
-       >> REAL_ARITH_TAC)
-   >> MATCH_MP_TAC PROB_SUBADDITIVE
-   >> RW_TAC std_ss [] >- PROVE_TAC []
-   >> MATCH_MP_TAC EVENTS_COUNTABLE_UNION
-   >> RW_TAC std_ss [SUBSET_DEF, IN_IMAGE, IN_COUNT, image_countable,
+  RW_TAC std_ss [SUBSET_DEF, IN_IMAGE, IN_UNIV,ext_suminf_def]
+  >> Suff `prob p (BIGUNION (IMAGE f UNIV)) = sup (IMAGE (prob p o (\n. BIGUNION (IMAGE f (count n)))) UNIV)`
+  >- (RW_TAC std_ss []
+      >> MATCH_MP_TAC sup_mono
+      >> RW_TAC std_ss [o_DEF]
+      >> Induct_on `n`
+      >- RW_TAC std_ss [COUNT_ZERO,IMAGE_EMPTY,BIGUNION_EMPTY,PROB_EMPTY,EXTREAL_SUM_IMAGE_EMPTY,le_refl]
+      >> RW_TAC std_ss [COUNT_SUC, IMAGE_INSERT, BIGUNION_INSERT]
+      >> (MP_TAC o Q.SPEC `n` o REWRITE_RULE [FINITE_COUNT,o_DEF] o Q.SPECL [`prob p o f`,`count n`] o INST_TYPE [alpha |-> ``:num``]) EXTREAL_SUM_IMAGE_PROPERTY
+      >> `(!x. x IN n INSERT count n ==> prob p (f x) <> NegInf)` by METIS_TAC [PROB_FINITE]
+      >> RW_TAC std_ss [COUNT_SUC]
+      >> `~(n < n)` by RW_TAC real_ss []
+      >> `count n DELETE n = count n` by METIS_TAC [DELETE_NON_ELEMENT,IN_COUNT]
+      >> RW_TAC std_ss []
+      >> `prob p (f n UNION BIGUNION (IMAGE f (count n))) <= prob p (f n) + prob p (BIGUNION (IMAGE f (count n)))`
+          by (MATCH_MP_TAC PROB_SUBADDITIVE
+              >> RW_TAC std_ss []
+              >- METIS_TAC []
+              >> MATCH_MP_TAC EVENTS_COUNTABLE_UNION
+              >> RW_TAC std_ss [SUBSET_DEF, IN_IMAGE, IN_COUNT, image_countable,
                      COUNTABLE_COUNT]
-   >> PROVE_TAC []);
+              >> METIS_TAC [])
+      >> METIS_TAC [le_ladd_imp,le_trans])
+  >> (MP_TAC o Q.SPECL [`p`,`(\n. BIGUNION (IMAGE f (count n)))`]) PROB_INCREASING_UNION
+  >> RW_TAC std_ss []
+  >> `BIGUNION (IMAGE (\n. BIGUNION (IMAGE f (count n))) UNIV) = BIGUNION (IMAGE f UNIV)`
+       by (RW_TAC std_ss [EXTENSION,IN_BIGUNION_IMAGE,IN_UNIV,IN_COUNT]
+           >> METIS_TAC [DECIDE ``x < SUC x``])
+  >> FULL_SIMP_TAC std_ss []
+  >> POP_ASSUM (K ALL_TAC)
+  >> POP_ASSUM (MATCH_MP_TAC o GSYM)
+  >> RW_TAC std_ss [IN_FUNSET,IN_UNIV]
+  >- (MATCH_MP_TAC EVENTS_COUNTABLE_UNION
+      >> RW_TAC std_ss [SUBSET_DEF, IN_IMAGE, IN_COUNT, image_countable,
+                        COUNTABLE_COUNT]
+      >> METIS_TAC [])
+  >> RW_TAC std_ss [SUBSET_DEF,IN_BIGUNION_IMAGE,IN_COUNT]
+  >> METIS_TAC [DECIDE ``n < SUC n``,LESS_TRANS]);
 
 val PROB_COUNTABLY_ZERO = store_thm
   ("PROB_COUNTABLY_ZERO",
@@ -557,73 +652,72 @@ val PROB_COUNTABLY_ZERO = store_thm
        prob_space p /\ countable c /\ c SUBSET events p /\
        (!x. x IN c ==> (prob p x = 0)) ==>
        (prob p (BIGUNION c) = 0)``,
-   RW_TAC std_ss [COUNTABLE_ENUM]
-   >- RW_TAC std_ss [BIGUNION_EMPTY, PROB_EMPTY]
-   >> Know `(!n. prob p (f n) = 0) /\ (!n. f n IN events p)`
-   >- (FULL_SIMP_TAC std_ss [IN_IMAGE, IN_UNIV, SUBSET_DEF]
-       >> PROVE_TAC [])
-   >> NTAC 2 (POP_ASSUM K_TAC)
-   >> STRIP_TAC
-   >> ONCE_REWRITE_TAC [GSYM REAL_LE_ANTISYM]
-   >> REVERSE CONJ_TAC
-   >- (MATCH_MP_TAC PROB_POSITIVE
-       >> RW_TAC std_ss []
-       >> MATCH_MP_TAC EVENTS_COUNTABLE_UNION
-       >> RW_TAC std_ss [COUNTABLE_IMAGE_NUM, SUBSET_DEF, IN_IMAGE, IN_UNIV]
-       >> RW_TAC std_ss [])
-   >> Know `(prob p o f) sums 0`
-   >- (Know `0 = sum (0, 0) (prob p o f)` >- RW_TAC std_ss [sum]
-       >> Rewr'
-       >> MATCH_MP_TAC SER_0
-       >> RW_TAC std_ss [o_THM])
-   >> RW_TAC std_ss [SUMS_EQ]
-   >> POP_ASSUM (REWRITE_TAC o wrap o SYM)
-   >> MATCH_MP_TAC PROB_COUNTABLY_SUBADDITIVE
-   >> RW_TAC std_ss [SUBSET_DEF, IN_IMAGE, IN_UNIV]
-   >> RW_TAC std_ss []);
+  RW_TAC std_ss [COUNTABLE_ENUM]
+  >- RW_TAC std_ss [BIGUNION_EMPTY, PROB_EMPTY]
+  >> Know `(!n. prob p (f n) = 0) /\ (!n. f n IN events p)`
+  >- (FULL_SIMP_TAC std_ss [IN_IMAGE, IN_UNIV, SUBSET_DEF]
+      >> PROVE_TAC [])
+  >> NTAC 2 (POP_ASSUM K_TAC)
+  >> STRIP_TAC
+  >> ONCE_REWRITE_TAC [GSYM le_antisym]
+  >> Reverse CONJ_TAC
+  >- (MATCH_MP_TAC PROB_POSITIVE
+      >> RW_TAC std_ss []
+      >> MATCH_MP_TAC EVENTS_COUNTABLE_UNION
+      >> RW_TAC std_ss [COUNTABLE_IMAGE_NUM, SUBSET_DEF, IN_IMAGE, IN_UNIV]
+      >> RW_TAC std_ss [])
+  >> Know `suminf (prob p o f) = 0`
+  >- RW_TAC std_ss [ext_suminf_def,o_DEF,EXTREAL_SUM_IMAGE_ZERO,FINITE_COUNT,
+                    sup_const_over_set,UNIV_NOT_EMPTY]
+  >> RW_TAC std_ss []
+  >> POP_ASSUM (REWRITE_TAC o wrap o SYM)
+  >> MATCH_MP_TAC PROB_COUNTABLY_SUBADDITIVE
+  >> RW_TAC std_ss [SUBSET_DEF, IN_IMAGE, IN_UNIV]
+  >> RW_TAC std_ss []);
 
 val INDEP_SYM = store_thm
   ("INDEP_SYM",
-   ``!p a b. prob_space p /\ indep p a b ==> indep p b a``,
+  ``!p a b. prob_space p /\ indep p a b ==> indep p b a``,
    RW_TAC std_ss [indep_def]
-   >> PROVE_TAC [REAL_MUL_SYM, INTER_COMM]);
+   >> PROVE_TAC [mul_comm, INTER_COMM]);
 
 val INDEP_REFL = store_thm
   ("INDEP_REFL",
    ``!p a.
        prob_space p /\ a IN events p ==>
        (indep p a a = (prob p a = 0) \/ (prob p a = 1))``,
-   RW_TAC std_ss [indep_def, INTER_IDEMPOT]
-   >> PROVE_TAC [REAL_MUL_IDEMPOT]);
-
+  RW_TAC std_ss [indep_def, INTER_IDEMPOT]
+  >> `?r. prob p a = Normal r` by METIS_TAC [PROB_FINITE,extreal_cases]
+  >> RW_TAC std_ss [extreal_mul_def,extreal_of_num_def,extreal_11]
+  >> METIS_TAC [REAL_MUL_IDEMPOT]);
 
 val PROB_REAL_SUM_IMAGE = store_thm
   ("PROB_REAL_SUM_IMAGE",
    ``!p s. prob_space p /\ s IN events p /\ (!x. x IN s ==> {x} IN events p) /\ FINITE s ==>
                 (prob p s = SIGMA (\x. prob p {x}) s)``,
-   Suff `!s. FINITE s ==>
+  Suff `!s. FINITE s ==>
         (\s. !p. prob_space p /\ s IN events p /\ (!x. x IN s ==> {x} IN events p) ==>
-                (prob p s = SIGMA (\x. prob p {x}) s)) s`
-   >- METIS_TAC []
-   >> MATCH_MP_TAC FINITE_INDUCT
-   >> RW_TAC std_ss [REAL_SUM_IMAGE_THM, PROB_EMPTY, DELETE_NON_ELEMENT, IN_INSERT]
-   >> Q.PAT_X_ASSUM `!p.
-            prob_space p /\ s IN events p /\
+             (prob p s = SIGMA (\x. prob p {x}) s)) s`
+  >- METIS_TAC []
+  >> MATCH_MP_TAC FINITE_INDUCT
+  >> RW_TAC std_ss [EXTREAL_SUM_IMAGE_EMPTY,PROB_EMPTY,IN_INSERT]
+  >> (MP_TAC o Q.SPEC `e` o UNDISCH o Q.SPECL [`(\x. prob p {x})`,`s`]) EXTREAL_SUM_IMAGE_PROPERTY
+  >> `!x. x IN e INSERT s ==> (\x. prob p {x}) x <> NegInf` by METIS_TAC [PROB_FINITE,IN_INSERT]
+  >> RW_TAC std_ss []
+  >> Q.PAT_X_ASSUM `!p. prob_space p /\ s IN events p /\
             (!x. x IN s ==> {x} IN events p) ==>
             (prob p s = SIGMA (\x. prob p {x}) s)` (MP_TAC o GSYM o Q.SPEC `p`)
-   >> RW_TAC std_ss []
-   >> `s IN events p`
-        by (`s = (e INSERT s) DIFF {e}`
-                by (RW_TAC std_ss [EXTENSION, IN_INSERT, IN_DIFF, IN_SING]
-                    >> METIS_TAC [GSYM DELETE_NON_ELEMENT])
-            >> POP_ORW
-            >> FULL_SIMP_TAC std_ss [prob_space_def, measure_space_def, sigma_algebra_def,
-                                     events_def]
-            >> METIS_TAC [space_def, subsets_def, ALGEBRA_DIFF])
-   >> ASM_SIMP_TAC std_ss []
-   >> MATCH_MP_TAC PROB_ADDITIVE
-   >> RW_TAC std_ss [IN_DISJOINT, IN_SING, Once INSERT_SING_UNION]
-   >> FULL_SIMP_TAC std_ss [GSYM DELETE_NON_ELEMENT]);
+  >> RW_TAC std_ss []
+  >> `s IN events p`
+      by (`s = (e INSERT s) DIFF {e}`
+             by (RW_TAC std_ss [EXTENSION, IN_INSERT, IN_DIFF, IN_SING] >> METIS_TAC [GSYM DELETE_NON_ELEMENT])
+          >> POP_ORW
+          >> FULL_SIMP_TAC std_ss [prob_space_def, measure_space_def, sigma_algebra_def, events_def]
+          >> METIS_TAC [space_def, subsets_def, ALGEBRA_DIFF])
+  >> FULL_SIMP_TAC std_ss [DELETE_NON_ELEMENT]
+  >> MATCH_MP_TAC PROB_ADDITIVE
+  >> RW_TAC std_ss [IN_DISJOINT, IN_SING, Once INSERT_SING_UNION]
+  >> FULL_SIMP_TAC std_ss [GSYM DELETE_NON_ELEMENT]);
 
 val PROB_EQUIPROBABLE_FINITE_UNIONS = store_thm
   ("PROB_EQUIPROBABLE_FINITE_UNIONS",
@@ -632,15 +726,15 @@ val PROB_EQUIPROBABLE_FINITE_UNIONS = store_thm
                 (prob p s = & (CARD s) * prob p {CHOICE s})``,
    RW_TAC std_ss []
    >> Cases_on `s = {}`
-   >- RW_TAC real_ss [PROB_EMPTY, CARD_EMPTY]
+   >- RW_TAC real_ss [PROB_EMPTY, CARD_EMPTY,mul_lzero]
    >> `prob p s = SIGMA (\x. prob p {x}) s`
         by METIS_TAC [PROB_REAL_SUM_IMAGE]
    >> POP_ORW
    >> `prob p {CHOICE s} = (\x. prob p {x}) (CHOICE s)` by RW_TAC std_ss []
    >> POP_ORW
-   >> (MATCH_MP_TAC o UNDISCH o Q.SPEC `s`) REAL_SUM_IMAGE_FINITE_SAME
-   >> RW_TAC std_ss [CHOICE_DEF]);
-
+   >> (MATCH_MP_TAC o UNDISCH o Q.SPEC `s`) EXTREAL_SUM_IMAGE_FINITE_SAME
+   >> RW_TAC std_ss [CHOICE_DEF]
+   >> METIS_TAC [PROB_FINITE]);
 
 val PROB_REAL_SUM_IMAGE_FN = store_thm
   ("PROB_REAL_SUM_IMAGE_FN",
@@ -650,7 +744,7 @@ val PROB_REAL_SUM_IMAGE_FN = store_thm
                 (BIGUNION (IMAGE f s) INTER p_space p = p_space p) ==>
                 (prob p e = SIGMA (\x. prob p (e INTER f x)) s)``,
    Suff `!(s :'b -> bool). FINITE s ==>
-        (\s. !(p :('a -> bool) # (('a -> bool) -> bool) # (('a -> bool) -> real))
+        (\s. !(p :('a -> bool) # (('a -> bool) -> bool) # (('a -> bool) -> extreal))
        (f :'b -> 'a -> bool) (e :'a -> bool). prob_space p /\ e IN events p /\
                 (!x. x IN s ==> e INTER f x IN events p) /\
                 (!x y. x IN s /\ y IN s /\ (~(x=y)) ==> DISJOINT (f x) (f y)) /\
@@ -658,9 +752,14 @@ val PROB_REAL_SUM_IMAGE_FN = store_thm
                 (prob p e = SIGMA (\x. prob p (e INTER f x)) s)) s`
    >- METIS_TAC []
    >> MATCH_MP_TAC FINITE_INDUCT
-   >> RW_TAC std_ss [REAL_SUM_IMAGE_THM, PROB_EMPTY, DELETE_NON_ELEMENT, IN_INSERT,
+   >> RW_TAC std_ss [EXTREAL_SUM_IMAGE_EMPTY, PROB_EMPTY, DELETE_NON_ELEMENT, IN_INSERT,
                      IMAGE_EMPTY, BIGUNION_EMPTY, INTER_EMPTY]
-   >- METIS_TAC [PROB_UNIV, PROB_EMPTY, REAL_10]
+   >- METIS_TAC [PROB_UNIV, PROB_EMPTY, REAL_10,extreal_of_num_def,extreal_11]
+   >> (MP_TAC o Q.SPEC `e` o UNDISCH o Q.SPECL [`(\x. prob p (e' INTER f x))`,`s`] o
+       INST_TYPE [alpha |-> beta]) EXTREAL_SUM_IMAGE_PROPERTY
+   >> `!x. x IN e INSERT s ==> (\x. prob p (e' INTER f x)) x <> NegInf`
+      by METIS_TAC [PROB_FINITE,IN_INSERT]
+   >> RW_TAC std_ss []
    >> `prob p e' =
         prob p (e' INTER f e) +
         prob p (e' DIFF f e)`
@@ -673,10 +772,10 @@ val PROB_REAL_SUM_IMAGE_FN = store_thm
                 FULL_SIMP_TAC std_ss [IN_DISJOINT, IN_INTER, IN_DIFF] >> METIS_TAC [],
                 RW_TAC std_ss [Once EXTENSION, IN_INTER, IN_UNION, IN_DIFF] >> DECIDE_TAC])
    >> POP_ORW
-   >> RW_TAC std_ss [REAL_EQ_LADD]
+   >> RW_TAC std_ss [EXTREAL_EQ_LADD,PROB_FINITE]
    >> (MP_TAC o Q.ISPEC `(s :'b -> bool)`) SET_CASES
    >> RW_TAC std_ss []
-   >- (RW_TAC std_ss [REAL_SUM_IMAGE_THM]
+   >- (RW_TAC std_ss [EXTREAL_SUM_IMAGE_EMPTY]
        >> `IMAGE f {e} = {f e}`
                 by RW_TAC std_ss [EXTENSION, IN_IMAGE, IN_SING]
        >> FULL_SIMP_TAC std_ss [BIGUNION_SING, DIFF_UNIV, PROB_EMPTY]
@@ -739,7 +838,15 @@ val PROB_REAL_SUM_IMAGE_FN = store_thm
    >> ASM_SIMP_TAC std_ss []
    >> STRIP_TAC >> POP_ASSUM (K ALL_TAC)
    >> FULL_SIMP_TAC std_ss [FINITE_INSERT]
-   >> RW_TAC std_ss [REAL_SUM_IMAGE_THM]
+   >> (MP_TAC o Q.SPEC `x` o UNDISCH o Q.SPECL [`(\x. prob p (e' INTER f x))`,`t`] o
+       INST_TYPE [alpha |-> beta]) EXTREAL_SUM_IMAGE_PROPERTY
+   >> `!x'. x' IN x INSERT t ==> (\x. prob p (e' INTER f x)) x' <> NegInf` by METIS_TAC [PROB_FINITE,IN_INSERT]
+   >> RW_TAC std_ss []
+   >> (MP_TAC o Q.SPEC `x` o UNDISCH o
+       Q.SPECL [`(\x'. prob p ((e' DIFF f e) INTER if x' = x then f x UNION f e else f x'))`,`t`] o
+       INST_TYPE [alpha |-> beta]) EXTREAL_SUM_IMAGE_PROPERTY
+   >> `!x'. x' IN x INSERT t ==> (\x'. prob p ((e' DIFF f e) INTER if x' = x then f x UNION f e else f x')) x' <> NegInf` by METIS_TAC [PROB_FINITE,IN_INSERT]
+   >> RW_TAC std_ss []
    >> FULL_SIMP_TAC std_ss [DELETE_NON_ELEMENT]
    >> FULL_SIMP_TAC std_ss [GSYM DELETE_NON_ELEMENT]
    >> `(e' DIFF f e) INTER (f x UNION f e) =
@@ -747,8 +854,10 @@ val PROB_REAL_SUM_IMAGE_FN = store_thm
         by (ONCE_REWRITE_TAC [EXTENSION] >> RW_TAC std_ss [IN_INTER, IN_DIFF, IN_UNION]
             >> FULL_SIMP_TAC std_ss [IN_DISJOINT, GSYM DELETE_NON_ELEMENT, IN_INSERT]
             >> METIS_TAC [])
-   >> RW_TAC std_ss [REAL_EQ_LADD]
-   >> ONCE_REWRITE_TAC [(UNDISCH o Q.ISPEC `(t :'b -> bool)`) REAL_SUM_IMAGE_IN_IF]
+   >> FULL_SIMP_TAC std_ss [EXTREAL_EQ_LADD,PROB_FINITE,IN_INSERT]
+   >> (MP_TAC o Q.SPEC `(\x. prob p (e' INTER f x))` o UNDISCH o Q.ISPEC `(t :'b -> bool)`) EXTREAL_SUM_IMAGE_IN_IF
+   >> (MP_TAC o Q.SPEC `(\x'. prob p ((e' DIFF f e) INTER if x' = x then f x UNION f e else f x'))` o UNDISCH o Q.ISPEC `(t :'b -> bool)`) EXTREAL_SUM_IMAGE_IN_IF
+   >> RW_TAC std_ss []
    >> Suff `(\x'.
          (if x' IN t then
             (\x'.
@@ -807,6 +916,7 @@ val PROB_DISCRETE_EVENTS_COUNTABLE = store_thm
           >> RW_TAC std_ss [EXTENSION,GSPECIFICATION,IN_IMAGE])
   >> METIS_TAC [EVENTS_COUNTABLE_UNION]);
 
+(* TODO:
 (* ************************************************************************* *)
 
 val marginal_joint_zero = store_thm
@@ -814,7 +924,7 @@ val marginal_joint_zero = store_thm
                             ((distribution p X s = 0) \/ (distribution p Y t = 0))
                              ==> (joint_distribution p X Y (s CROSS t) = 0)``,
   RW_TAC std_ss [joint_distribution_def,distribution_def]
-  >- ( `PREIMAGE (\x. (X x,Y x)) (s CROSS t) INTER p_space p SUBSET (PREIMAGE X s INTER p_space p)`
+  >- (`PREIMAGE (\x. (X x,Y x)) (s CROSS t) INTER p_space p SUBSET (PREIMAGE X s INTER p_space p)`
       by RW_TAC std_ss [SUBSET_DEF,IN_PREIMAGE,IN_INTER,IN_CROSS]
   >> `prob p (PREIMAGE (\x. (X x,Y x)) (s CROSS t) INTER p_space p) <= prob p (PREIMAGE X s INTER p_space p)`
        by METIS_TAC [PROB_INCREASING,INTER_SUBSET,IN_POW]
@@ -864,7 +974,7 @@ val distribution_prob_space = store_thm
             f IN (UNIV -> measurable_sets p) /\
             (!m n. ~(m = n) ==> DISJOINT (f m) (f n)) /\
             BIGUNION (IMAGE f UNIV) IN measurable_sets p ==>
-            measure p o f sums measure p (BIGUNION (IMAGE f univ(:num)))`
+            (measure p (BIGUNION (IMAGE f univ(:num))) = suminf (measure p o f))`
                 (MP_TAC o Q.SPEC `(\x. PREIMAGE X x INTER p_space p) o f`)
        >> RW_TAC std_ss [prob_def, o_DEF, PREIMAGE_BIGUNION, IMAGE_IMAGE]
        >> `(BIGUNION (IMAGE (\x. PREIMAGE X (f x)) UNIV) INTER p_space p) =
@@ -946,8 +1056,7 @@ val distribution_partition = store_thm
 val distribution_lebesgue_thm1 = store_thm
   ("distribution_lebesgue_thm1",
    ``!X p s A. random_variable X p s /\ A IN subsets s ==>
-             (Normal(distribution p X A) =
-              integral p (indicator_fn (PREIMAGE X A INTER p_space p)))``,
+             (distribution p X A = integral p (indicator_fn (PREIMAGE X A INTER p_space p)))``,
    RW_TAC std_ss [random_variable_def, prob_space_def, distribution_def, events_def,
                   IN_MEASURABLE,p_space_def, prob_def, subsets_def, space_def,
                   GSYM integral_indicator]);
@@ -955,32 +1064,32 @@ val distribution_lebesgue_thm1 = store_thm
 val distribution_lebesgue_thm2 = store_thm
   ("distribution_lebesgue_thm2",
    ``!X p s A. random_variable X p s /\ A IN subsets s ==>
-        (Normal (distribution p X A) =
-         integral (space s, subsets s, distribution p X) (indicator_fn A))``,
+             (distribution p X A = integral (space s, subsets s, distribution p X) (indicator_fn A))``,
    REPEAT STRIP_TAC
    >> `prob_space (space s,subsets s,distribution p X)`
         by RW_TAC std_ss [distribution_prob_space]
    >> Q.PAT_X_ASSUM `random_variable X p s` MP_TAC
-   >> RW_TAC std_ss [random_variable_def,prob_space_def,distribution_def,events_def,IN_MEASURABLE,p_space_def,
-                     prob_def,subsets_def, space_def]
+   >> RW_TAC std_ss [random_variable_def, prob_space_def, distribution_def, events_def, IN_MEASURABLE, p_space_def, prob_def,
+                  subsets_def, space_def]
    >> `measure p (PREIMAGE X A INTER m_space p) =
        measure (space s,subsets s,(\A. measure p (PREIMAGE X A INTER m_space p))) A`
         by RW_TAC std_ss [measure_def]
    >> POP_ORW
-   >> (MP_TAC o Q.SPECL [`(space s,subsets s,(\A. measure p (PREIMAGE X A INTER m_space p)))`,`A`] o
-       INST_TYPE [``:'a``|->``:'b``]) integral_indicator
+   >> (MP_TAC o Q.SPECL [`(space s,subsets s,(\A. measure p (PREIMAGE X A INTER m_space p)))`,`A`] o INST_TYPE [``:'a``|->``:'b``])
+        integral_indicator
    >> FULL_SIMP_TAC std_ss [measurable_sets_def, prob_space_def, distribution_def, prob_def, p_space_def]);
+
+(* ************************************************************************* *)
 
 val finite_expectation1 = store_thm
   ("finite_expectation1",
    ``!p X. FINITE (p_space p) /\ real_random_variable X p ==>
                 (expectation p X =
-                 SIGMA (\r. r * Normal (prob p (PREIMAGE X {r} INTER p_space p)))
+                 SIGMA (\r. r * prob p (PREIMAGE X {r} INTER p_space p))
                        (IMAGE X (p_space p)))``,
-   RW_TAC std_ss [expectation_def, p_space_def, prob_def, prob_space_def,
-                  real_random_variable_def, events_def]
+   RW_TAC std_ss [expectation_def, p_space_def, prob_def, prob_space_def, real_random_variable_def, events_def]
    >> (MATCH_MP_TAC o REWRITE_RULE [finite_space_integral_def]) finite_space_integral_reduce
-   >> RW_TAC std_ss [num_not_infty]);
+   >> RW_TAC std_ss []);
 
 val finite_expectation2 = store_thm
   ("finite_expectation2",
@@ -996,7 +1105,9 @@ val finite_expectation2 = store_thm
 val finite_expectation = store_thm
   ("finite_expectation",
    ``!p X. FINITE (p_space p) /\ real_random_variable X p ==>
-        (expectation p X = SIGMA (\r. r * Normal (distribution p X {r})) (IMAGE X (p_space p)))``,
+                (expectation p X =
+                 SIGMA (\r. r * distribution p X {r})
+                       (IMAGE X (p_space p)))``,
    RW_TAC std_ss [distribution_def]
    >> METIS_TAC [finite_expectation1]);
 
@@ -1130,7 +1241,7 @@ val distribution_x_eq_1_imp_distribution_y_eq_0 = store_thm
            (p_space
               (p :
                 ('a -> bool) #
-                (('a -> bool) -> bool) # (('a -> bool) -> real))),
+                (('a -> bool) -> bool) # (('a -> bool) -> extreal))),
          POW (IMAGE X (p_space p)),distribution p X)`,
                         `x:'b`]) prob_x_eq_1_imp_prob_y_eq_0
    >> SIMP_TAC std_ss [EVENTS, IN_POW, SUBSET_DEF, IN_SING, PROB]
@@ -1140,7 +1251,7 @@ val distribution_x_eq_1_imp_distribution_y_eq_0 = store_thm
             >> `PREIMAGE X {x} INTER p_space p = {}`
                 by (RW_TAC std_ss [Once EXTENSION, IN_INTER, IN_SING, IN_PREIMAGE, NOT_IN_EMPTY]
                     >> METIS_TAC [])
-            >> METIS_TAC [random_variable_def, PROB_EMPTY, EVAL ``0 <> 1:real``])
+            >> METIS_TAC [random_variable_def, PROB_EMPTY, ne_01])
    >> POP_ORW
    >> RW_TAC std_ss []
    >> Cases_on `y IN IMAGE X (p_space p)` >- ASM_SIMP_TAC std_ss []
@@ -1344,5 +1455,30 @@ val joint_distribution_sum_mul1 = store_thm
   >> Suff `(\x. (f x) * distribution p X {x}) = (\x. distribution p X {x} * (f x))`
   >- RW_TAC std_ss []
   >> RW_TAC std_ss [FUN_EQ_THM, REAL_MUL_COMM]);
+*)
+
+(******************************************************************************)
+(*  Kolmogorov's 0-1 Law                                                      *)
+(******************************************************************************)
+
+val tail_events_def = Define (* or "remote_events" *)
+   `tail_events (p :'a p_space) (A :num -> 'a events) =
+      BIGINTER (IMAGE (\n. subsets (sigma (p_space p)
+                                          (BIGUNION (IMAGE A {m | m > n}))))
+                      univ(:num))`;
+
+val kolmogorov_0_1_law = store_thm (* [3, p.37-38] *)
+  ("kolmogorov_0_1_law",
+  ``!(p :'a p_space) (A :num -> 'a events).
+       (!n. sigma_algebra (p_space p, E n)) /\ indep_sets p A UNIV ==>
+        !e. e IN tail_events p A ==> (prob p e = 0) \/ (prob p e = 1)``,
+    cheat);
 
 val _ = export_theory ();
+
+(* References:
+
+  [1] Kolmogorov, A.N.: Foundations of the Theory of Probability. Chelsea Publishing Company, New York, N. Y. (1950).
+  [2] Chung, K.L.: A Course in Probability Theory, Third Edition. Academic Press (2001).
+  [3] Rosenthal, J.S.: A First Look at Rigorous Probability Theory. World Scientific Publishing Company (2006).
+ *)
