src/probability/martingaleScript.sml
@@ -1,0 +1,294 @@
+(* ------------------------------------------------------------------------- *)
+(* The theory of martingales for sigma-finite measure spaces [1]             *)
+(*                                                                           *)
+(* Author: Chun Tian (2019)                                                  *)
+(* Fondazione Bruno Kessler and University of Trento, Italy                  *)
+(* ------------------------------------------------------------------------- *)
+
+open HolKernel Parse boolLib bossLib;
+open arithmeticTheory realTheory prim_recTheory pairTheory relationTheory
+     seqTheory pred_setTheory res_quanTheory res_quanTools transcTheory
+     pairTheory combinTheory realLib optionTheory real_sigmaTheory;
+
+open hurdUtils util_probTheory extrealTheory measureTheory lebesgueTheory;
+
+val _ = new_theory "martingale";
+
+(* "The theory of martingales as we know it now goes back to
+    Doob and most of the material of this and the following chapter can be found in
+    his seminal monograph [2] from 1953.
+
+    We want to understand martingales as an analysis tool which will be useful
+    for the study of L^p- and almost everywhere convergence and, in particular,
+    for the further development of measure and integration theory. Our presentation
+    differs somewhat from the standard way to introduce martingales - conditional
+    expectations will be defined later in Chapter 22 - but the results and their
+    proofs are pretty much the usual ones."
+
+  -- Rene L. Schilling, Measures, Integrals and Martingales [1] *)
+
+(* ------------------------------------------------------------------------- *)
+(*  Basic version of martingales (Chapter 17 of [1])                         *)
+(* ------------------------------------------------------------------------- *)
+
+val sub_sigma_algebra_def = Define
+   `sub_sigma_algebra a b = sigma_algebra a /\ sigma_algebra b /\
+                           (space a = space b) /\ (subsets a) SUBSET (subsets b)`;
+
+(* sub_sigma_algebra is a partial-order between sigma-algebras *)
+val SUB_SIGMA_ALGEBRA_REFL = store_thm
+  ("SUB_SIGMA_ALGEBRA_REFL",
+  ``!a. sigma_algebra a ==> sub_sigma_algebra a a``,
+    RW_TAC std_ss [sub_sigma_algebra_def, SUBSET_REFL]);
+
+val SUB_SIGMA_ALGEBRA_TRANS = store_thm
+  ("SUB_SIGMA_ALGEBRA_TRANS",
+  ``!a b c. sub_sigma_algebra a b /\ sub_sigma_algebra b c ==> sub_sigma_algebra a c``,
+    RW_TAC std_ss [sub_sigma_algebra_def]
+ >> MATCH_MP_TAC SUBSET_TRANS
+ >> Q.EXISTS_TAC `subsets b` >> art []);
+
+val SUB_SIGMA_ALGEBRA_ANTISYM = store_thm
+  ("SUB_SIGMA_ALGEBRA_ANTISYM",
+  ``!a b. sub_sigma_algebra a b /\ sub_sigma_algebra b a ==> (a = b)``,
+    RW_TAC std_ss [sub_sigma_algebra_def]
+ >> Q.PAT_X_ASSUM `space b = space a` K_TAC
+ >> ONCE_REWRITE_TAC [GSYM SPACE]
+ >> ASM_REWRITE_TAC [CLOSED_PAIR_EQ]
+ >> MATCH_MP_TAC SUBSET_ANTISYM >> art []);
+
+val SUB_SIGMA_ALGEBRA_ORDER = store_thm
+  ("SUB_SIGMA_ALGEBRA_ORDER", ``Order sub_sigma_algebra``,
+    RW_TAC std_ss [Order, antisymmetric_def, transitive_def]
+ >- (MATCH_MP_TAC SUB_SIGMA_ALGEBRA_ANTISYM >> art [])
+ >> IMP_RES_TAC SUB_SIGMA_ALGEBRA_TRANS);
+
+val SUB_SIGMA_ALGEBRA_MEASURE_SPACE = store_thm
+  ("SUB_SIGMA_ALGEBRA_MEASURE_SPACE",
+  ``!m a. measure_space m /\ sub_sigma_algebra a (m_space m,measurable_sets m) ==>
+          measure_space (m_space m,subsets a,measure m)``,
+    RW_TAC std_ss [sub_sigma_algebra_def, space_def, subsets_def]
+ >> MATCH_MP_TAC MEASURE_SPACE_RESTRICTION
+ >> Q.EXISTS_TAC `measurable_sets m`
+ >> simp [MEASURE_SPACE_REDUCE]
+ >> METIS_TAC [SPACE]);
+
+(* `filtration A` is the set of all filtrations of A *)
+val filtration_def = Define
+   `filtration A (a :num -> 'a algebra) =
+      (!n. sub_sigma_algebra (a n) A) /\
+      (!i j. i <= j ==> subsets (a i) SUBSET subsets (a j))`;
+
+val FILTRATION_BOUNDED = store_thm
+  ("FILTRATION_BOUNDED",
+  ``!A a. filtration A a ==> !n. sub_sigma_algebra (a n) A``,
+    PROVE_TAC [filtration_def]);
+
+val FILTRATION_MONO = store_thm
+  ("FILTRATION_MONO",
+  ``!A a. filtration A a ==> !i j. i <= j ==> subsets (a i) SUBSET subsets (a j)``,
+    PROVE_TAC [filtration_def]);
+
+(* all sigma-algebras in `filtration A` are subset of A *)
+val FILTRATION_SUBSETS = store_thm
+  ("FILTRATION_SUBSETS",
+  ``!A a. filtration A a ==> !n. subsets (a n) SUBSET (subsets A)``,
+    RW_TAC std_ss [filtration_def, sub_sigma_algebra_def]);
+
+val FILTRATION = store_thm
+  ("FILTRATION",
+  ``!A a. filtration A a = (!n. sub_sigma_algebra (a n) A) /\
+                           (!n. subsets (a n) SUBSET (subsets A)) /\
+                           (!i j. i <= j ==> subsets (a i) SUBSET subsets (a j))``,
+    rpt GEN_TAC >> EQ_TAC
+ >- (DISCH_TAC >> IMP_RES_TAC FILTRATION_SUBSETS \\
+     fs [filtration_def])
+ >> RW_TAC std_ss [filtration_def]);
+
+val filtered_measure_space_def = Define
+   `filtered_measure_space (sp,sts,m) a =
+             measure_space (sp,sts,m) /\ filtration (sp,sts) a`;
+
+(* `sigma_finite_FMS = sigma_finite_filtered_measure_space` *)
+val sigma_finite_filtered_measure_space_def = Define
+   `sigma_finite_filtered_measure_space (sp,sts,m) a =
+                 filtered_measure_space (sp,sts,m) a /\ sigma_finite (sp,subsets (a 0),m)`;
+
+(* a shorter abbreviation *)
+val _ = overload_on ("sigma_finite_FMS",
+                    ``sigma_finite_filtered_measure_space``);
+
+val sigma_finite_FMS_def =
+    sigma_finite_filtered_measure_space_def;
+
+(* all sub measure spaces of a sigma-finite fms are also sigma-finite *)
+val SIGMA_FINITE_FMS_IMP = store_thm
+  ("SIGMA_FINITE_FMS_IMP",
+  ``!sp sts a m. sigma_finite_FMS (sp,sts,m) a ==> !n. sigma_finite (sp,subsets (a n),m)``,
+ (* proof *)
+    RW_TAC std_ss [sigma_finite_FMS_def, filtered_measure_space_def, filtration_def]
+ >> Know `measure_space (sp,subsets (a 0),m) /\
+          measure_space (sp,subsets (a n),m)`
+ >- (CONJ_TAC \\ (* 2 subgoals, same tactics *)
+     MATCH_MP_TAC (REWRITE_RULE [m_space_def, measurable_sets_def, measure_def]
+                                (Q.SPEC `(sp,sts,m)` SUB_SIGMA_ALGEBRA_MEASURE_SPACE)) >> art [])
+ >> STRIP_TAC
+ >> POP_ASSUM (simp o wrap o (MATCH_MP SIGMA_FINITE_ALT))
+ >> POP_ASSUM (fs o wrap o (MATCH_MP SIGMA_FINITE_ALT))
+ >> Q.EXISTS_TAC `f`
+ >> fs [IN_FUNSET, IN_UNIV, measurable_sets_def, m_space_def, measure_def]
+ >> `0 <= n` by RW_TAC arith_ss []
+ >> METIS_TAC [SUBSET_DEF]);
+
+(* extended definition *)
+val SIGMA_FINITE_FMS = store_thm
+  ("SIGMA_FINITE_FMS",
+  ``!sp sts a m. sigma_finite_FMS (sp,sts,m) a =
+                 filtered_measure_space (sp,sts,m) a /\
+                 !n. sigma_finite (sp,subsets (a n),m)``,
+    rpt GEN_TAC >> EQ_TAC
+ >- (DISCH_TAC >> IMP_RES_TAC SIGMA_FINITE_FMS_IMP \\
+     fs [sigma_finite_FMS_def])
+ >> RW_TAC std_ss [sigma_finite_FMS_def]);
+
+(* the smallest sigma-algebra generated by all (a n) *)
+val infty_sigma_algebra_def = Define
+   `infty_sigma_algebra sp a = sigma sp (BIGUNION (IMAGE (\(i :num). subsets (a i)) UNIV))`;
+
+val INFTY_SIGMA_ALGEBRA_BOUNDED = store_thm
+  ("INFTY_SIGMA_ALGEBRA_BOUNDED",
+  ``!A a. filtration A a ==> sub_sigma_algebra (infty_sigma_algebra (space A) a) A``,
+    RW_TAC std_ss [sub_sigma_algebra_def, FILTRATION, infty_sigma_algebra_def]
+ >- (MATCH_MP_TAC SIGMA_ALGEBRA_SIGMA \\
+     RW_TAC std_ss [subset_class_def, IN_BIGUNION_IMAGE, IN_UNIV] \\
+    `x IN subsets A` by PROVE_TAC [SUBSET_DEF] \\
+     METIS_TAC [sigma_algebra_def, algebra_def, subset_class_def, space_def, subsets_def])
+ >- REWRITE_TAC [SPACE_SIGMA]
+ >> MATCH_MP_TAC SIGMA_SUBSET >> art []
+ >> RW_TAC std_ss [SUBSET_DEF, IN_BIGUNION_IMAGE, IN_UNIV]
+ >> PROVE_TAC [SUBSET_DEF]);
+
+val INFTY_SIGMA_ALGEBRA_MAXIMAL = store_thm
+  ("INFTY_SIGMA_ALGEBRA_MAXIMAL",
+  ``!A a. filtration A a ==> !n. sub_sigma_algebra (a n) (infty_sigma_algebra (space A) a)``,
+    RW_TAC std_ss [sub_sigma_algebra_def, FILTRATION, infty_sigma_algebra_def]
+ >- (MATCH_MP_TAC SIGMA_ALGEBRA_SIGMA \\
+     RW_TAC std_ss [subset_class_def, IN_BIGUNION_IMAGE, IN_UNIV] \\
+    `x IN subsets A` by PROVE_TAC [SUBSET_DEF] \\
+     METIS_TAC [sigma_algebra_def, algebra_def, subset_class_def, space_def, subsets_def])
+ >- REWRITE_TAC [SPACE_SIGMA]
+ >> MATCH_MP_TAC SUBSET_TRANS
+ >> Q.EXISTS_TAC `BIGUNION (IMAGE (\i. subsets (a i)) univ(:num))`
+ >> CONJ_TAC
+ >- (RW_TAC std_ss [SUBSET_DEF, IN_BIGUNION_IMAGE, IN_UNIV] \\
+     Q.EXISTS_TAC `n` >> art [])
+ >> REWRITE_TAC [SIGMA_SUBSET_SUBSETS]);
+
+(* `prob_martingale` will be the probability version of `martingale` *)
+val martingale_def = Define
+   `martingale m a u =
+      sigma_finite_FMS m a /\ (!n. integrable m (u n)) /\
+      !n s. s IN (subsets (a n)) ==>
+           (integral m (\x. u (SUC n) x * indicator_fn s x) =
+            integral m (\x. u n x * indicator_fn s x))`;
+
+val super_martingale_def = Define
+   `super_martingale m a u =
+      sigma_finite_FMS m a /\ (!n. integrable m (u n)) /\
+      !n s. s IN (subsets (a n)) ==>
+           (integral m (\x. u (SUC n) x * indicator_fn s x) <=
+            integral m (\x. u n x * indicator_fn s x))`;
+
+val sub_martingale_def = Define
+   `sub_martingale m a u =
+      sigma_finite_FMS m a /\ (!n. integrable m (u n)) /\
+      !n s. s IN (subsets (a n)) ==>
+           (integral m (\x. u n x * indicator_fn s x) <=
+            integral m (\x. u (SUC n) x * indicator_fn s x))`;
+
+(* u is a martingale if, and only if, it is both a sub- and a supermartingale *)
+val MARTINGALE_BOTH_SUB_SUPER = store_thm
+  ("MARTINGALE_BOTH_SUB_SUPER",
+  ``!m a u. martingale m a u = sub_martingale m a u /\ super_martingale m a u``,
+    RW_TAC std_ss [martingale_def, sub_martingale_def, super_martingale_def]
+ >> EQ_TAC >> RW_TAC std_ss [le_refl]
+ >> ASM_SIMP_TAC std_ss [GSYM le_antisym]);
+
+(* ------------------------------------------------------------------------- *)
+(*  General version of martingales with poset indexes (Chapter 19 of [1])    *)
+(* ------------------------------------------------------------------------- *)
+
+open posetTheory;
+
+val POSET_NUM_LE = store_thm
+  ("POSET_NUM_LE", ``poset (univ(:num),$<=)``,
+    RW_TAC std_ss [poset_def]
+ >- (Q.EXISTS_TAC `0` >> REWRITE_TAC [GSYM IN_APP, IN_UNIV])
+ >- (MATCH_MP_TAC LESS_EQUAL_ANTISYM >> art [])
+ >> MATCH_MP_TAC LESS_EQ_TRANS
+ >> Q.EXISTS_TAC `y` >> art []);
+
+(* below J is an index set, R is a partial order on J *)
+val filtration_I_def = Define
+   `filtration_I A a (J,R) =
+      poset (J,R) /\ (!n. n IN J ==> sub_sigma_algebra (a n) A) /\
+      (!i j. i IN J /\ j IN J /\ R i j ==> subsets (a i) SUBSET subsets (a j))`;
+
+val FILTRATION_ALT = store_thm
+  ("FILTRATION_ALT",
+  ``!A a. filtration A a = filtration_I A a (univ(:num),$<=)``,
+    RW_TAC std_ss [filtration_def, filtration_I_def, POSET_NUM_LE, IN_UNIV]);
+
+val filtered_measure_space_I_def = Define
+   `filtered_measure_space_I (sp,sts,m) a (J,R) =
+             measure_space (sp,sts,m) /\ filtration_I (sp,sts) a (J,R)`;
+
+val FILTERED_MEASURE_SPACE_ALT = store_thm
+  ("FILTERED_MEASURE_SPACE_ALT",
+  ``!sp sts m a. filtered_measure_space (sp,sts,m) a =
+                 filtered_measure_space_I (sp,sts,m) a (univ(:num),$<=)``,
+    RW_TAC std_ss [filtered_measure_space_def, filtered_measure_space_I_def,
+                   FILTRATION_ALT, POSET_NUM_LE, IN_UNIV]);
+
+val sigma_finite_filtered_measure_space_I_def = Define
+   `sigma_finite_filtered_measure_space_I (sp,sts,m) a (J,R) =
+          filtered_measure_space_I (sp,sts,m) a (J,R) /\
+          !n. n IN J ==> sigma_finite (sp,subsets (a n),m)`;
+
+(* a shorter abbreviation *)
+val _ = overload_on ("sigma_finite_FMS_I",
+                    ``sigma_finite_filtered_measure_space_I``);
+
+val sigma_finite_FMS_I_def =
+    sigma_finite_filtered_measure_space_I_def;
+
+val SIGMA_FINITE_FMS_ALT = store_thm
+  ("SIGMA_FINITE_FMS_ALT",
+  ``!sp sts m a. sigma_finite_FMS (sp,sts,m) a =
+                 sigma_finite_FMS_I (sp,sts,m) a (univ(:num),$<=)``,
+    RW_TAC std_ss [SIGMA_FINITE_FMS, sigma_finite_FMS_I_def,
+                   FILTERED_MEASURE_SPACE_ALT, IN_UNIV]);
+
+val infty_sigma_algebra_I_def = Define
+   `infty_sigma_algebra_I sp a I = sigma sp (BIGUNION (IMAGE (\i. subsets (a i)) I))`;
+
+(* `martingale_I m a u (univ(:num),$<=) = martingale m a u` *)
+val martingale_I_def = Define
+   `martingale_I m a u (J,R) =
+      sigma_finite_FMS_I m a (J,R) /\ (!n. n IN J ==> integrable m (u n)) /\
+      !i j s. i IN J /\ j IN J /\ R i j /\ s IN (subsets (a i)) ==>
+           (integral m (\x. u i x * indicator_fn s x) =
+            integral m (\x. u j x * indicator_fn s x))`;
+
+(* or "upwards directed" *)
+val upwards_filtering_def = Define
+   `upwards_filtering (J,R) =
+      !a b. a IN J /\ b IN J ==> ?c. c IN J /\ R a c /\ R b c`;
+
+val _ = export_theory ();
+
+(* References:
+
+  [1] Schilling, R.L.: Measures, Integrals and Martingales. Cambridge University Press (2005).
+  [2] Doob, J.L.: Stochastic processes. Wiley-Interscience (1990).
+ *)
