src/probability/util_probScript.sml
@@ -5,44 +5,10 @@
 (* ------------------------------------------------------------------------- *)
 
 open HolKernel Parse boolLib bossLib metisLib combinTheory pred_setTheory seqTheory
-     res_quanTools pairTheory arithmeticTheory realTheory realLib transcTheory
-     real_sigmaTheory;
+     pairTheory arithmeticTheory realTheory realLib transcTheory
+     real_sigmaTheory hurdUtils;
 
 val _ = new_theory "util_prob";
-
-val S_TAC = rpt (POP_ASSUM MP_TAC) >> rpt RESQ_STRIP_TAC;
-val Strip = S_TAC;
-
-fun K_TAC _ = ALL_TAC;
-val KILL_TAC = POP_ASSUM_LIST K_TAC;
-val Know = Q_TAC KNOW_TAC;
-val Suff = Q_TAC SUFF_TAC;
-val POP_ORW = POP_ASSUM (fn thm => ONCE_REWRITE_TAC [thm]);
-
-val Cond =
-  MATCH_MP_TAC (PROVE [] ``!a b c. a /\ (b ==> c) ==> ((a ==> b) ==> c)``)
-  >> CONJ_TAC;
-
-local
-  val th = prove (``!a b. a /\ (a ==> b) ==> a /\ b``, PROVE_TAC [])
-in
-  val STRONG_CONJ_TAC :tactic = MATCH_MP_TAC th >> CONJ_TAC
-end;
-
-fun wrap a = [a];
-val Rewr = DISCH_THEN (REWRITE_TAC o wrap);
-val Rewr' = DISCH_THEN (ONCE_REWRITE_TAC o wrap);
-val std_ss' = std_ss ++ boolSimps.ETA_ss
-
-
-(* ------------------------------------------------------------------------- *)
-(* Auxiliary theorems.                                                       *)
-(* ------------------------------------------------------------------------- *)
-
-val EQ_T_IMP = store_thm
-  ("EQ_T_IMP",
-   ``!x. x = T ==> x``,
-   PROVE_TAC []);
 
 (* ------------------------------------------------------------------------- *)
 (* bool theory subtypes.                                                     *)
@@ -50,15 +16,16 @@ val EQ_T_IMP = store_thm
 
 (* Subtype definitions *)
 
-val _ = add_infix("->", 250, HOLgrammars.RIGHT);
+val _ = add_infix ("->", 250, HOLgrammars.RIGHT);
 
-val _ = overload_on
-  ("->", ``FUNSET:('a->bool) -> ('b->bool) -> (('a->'b)->bool)``);
-val _ = overload_on
-  ("-->", ``DFUNSET : ('a->bool) -> ('a->'b->bool) -> (('a->'b)->bool)``);
+val _ = overload_on ("->",
+      ``FUNSET  :'a set -> 'b set -> ('a -> 'b) set``);
+
+val _ = overload_on ("-->", (* "Pi" in Isabelle's FuncSet.thy *)
+      ``DFUNSET :'a set -> ('a -> 'b set) -> ('a -> 'b) set``);
 
 val pair_def = Define
-  `pair (X : 'a -> bool) (Y : 'b -> bool) = \ (x, y). x IN X /\ y IN Y`;
+   `pair (X :'a -> bool) (Y :'b -> bool) = \(x, y). x IN X /\ y IN Y`;
 
 val IN_PAIR = store_thm
   ("IN_PAIR",
@@ -68,7 +35,7 @@ val IN_PAIR = store_thm
 
 val PAIR_UNIV = store_thm
   ("PAIR_UNIV",
-   ``pair UNIV UNIV = (UNIV : 'a # 'b -> bool)``,
+   ``pair UNIV UNIV = (UNIV :'a # 'b -> bool)``,
    RW_TAC std_ss [EXTENSION,GSPECIFICATION, IN_PAIR, IN_UNIV]);
 
 val PAIRED_BETA_THM = store_thm
@@ -177,9 +144,6 @@ val lg_pow = store_thm
             >> RW_TAC real_ss [LN_POS, LN_MONO_LT])
    >> RW_TAC real_ss [real_div, GSYM REAL_MUL_ASSOC, REAL_MUL_RINV]);
 
-
-
-(********************************************************************************************)
 (********************************************************************************************)
 
 val NUM_2D_BIJ = store_thm
@@ -290,12 +254,35 @@ val NUM_2D_BIJ_NZ_ALT2_INV = store_thm
        (((UNIV : num -> bool) DIFF {0}) CROSS ((UNIV : num -> bool) DIFF {0}))``,
    PROVE_TAC [NUM_2D_BIJ_NZ_ALT2, BIJ_SYM]);
 
-val prod_sets_def = Define `prod_sets a b = {s CROSS t | s IN a /\ t IN b}`;
+(* Two NUM_2D_BIJ concrete lemmas related to numpairTheory *)
+open numpairTheory;
+
+val NUM_2D_BIJ_nfst_nsnd = store_thm
+  ("NUM_2D_BIJ_nfst_nsnd", ``BIJ (\n. (nfst n, nsnd n)) UNIV (UNIV CROSS UNIV)``,
+    REWRITE_TAC [BIJ_ALT, IN_CROSS, IN_FUNSET, IN_UNIV]
+ >> BETA_TAC >> GEN_TAC >> Cases_on `y`
+ >> SIMP_TAC std_ss [EXISTS_UNIQUE_ALT]
+ >> Q.EXISTS_TAC `npair q r`
+ >> GEN_TAC >> STRIP_ASSUME_TAC (Q.SPEC `x'` npair_cases)
+ >> POP_ASSUM (REWRITE_TAC o wrap)
+ >> REWRITE_TAC [nfst_npair, nsnd_npair, npair_11]);
+
+val NUM_2D_BIJ_npair = store_thm
+  ("NUM_2D_BIJ_npair", ``BIJ (UNCURRY npair) (UNIV CROSS UNIV) UNIV``,
+    REWRITE_TAC [BIJ_ALT, IN_CROSS, IN_FUNSET, IN_UNIV, UNCURRY]
+ >> GEN_TAC >> SIMP_TAC std_ss [EXISTS_UNIQUE_ALT]
+ >> Q.EXISTS_TAC `nfst y, nsnd y`
+ >> GEN_TAC >> STRIP_ASSUME_TAC (Q.SPEC `y` npair_cases)
+ >> POP_ASSUM (REWRITE_TAC o wrap)
+ >> REWRITE_TAC [nfst_npair, nsnd_npair, npair_11]
+ >> Cases_on `x'` >> SIMP_TAC std_ss []);
+
+val prod_sets_def = Define `
+    prod_sets a b = {s CROSS t | s IN a /\ t IN b}`;
 
 val IN_o = store_thm
-  ("IN_o",
-   ``!x f s. x IN (s o f) = f x IN s``,
-   RW_TAC std_ss [SPECIFICATION, o_THM]);
+  ("IN_o", ``!x f s. x IN (s o f) = f x IN s``,
+    RW_TAC std_ss [SPECIFICATION, o_THM]);
 
 val IN_PROD_SETS = store_thm
   ("IN_PROD_SETS",
@@ -732,19 +719,9 @@ val MINIMAL_SUC_IMP = store_thm
    PROVE_TAC [MINIMAL_SUC]);
 
 (* ------------------------------------------------------------------------- *)
-(*   Disjoint subsets (from lebesgue_measureTheory)                          *)
+(*   Disjoint subsets (from HVG's lebesgue_measureTheory)                    *)
 (* ------------------------------------------------------------------------- *)
 
-fun SET_TAC L =
-    POP_ASSUM_LIST (K ALL_TAC) THEN REPEAT COND_CASES_TAC \\
-    REWRITE_TAC (append [EXTENSION, SUBSET_DEF, PSUBSET_DEF, DISJOINT_DEF,
-                         SING_DEF] L) \\
-    SIMP_TAC std_ss [NOT_IN_EMPTY, IN_UNIV, IN_UNION, IN_INTER, IN_DIFF,
-                     IN_INSERT, IN_DELETE, IN_REST, IN_BIGINTER, IN_BIGUNION,
-                     IN_IMAGE, GSPECIFICATION, IN_DEF, EXISTS_PROD, IN_FUNSET] \\
-    METIS_TAC [];
-
-(* moved here from lebesgue_measureTheory *)
 val disjoint_def = Define
    `disjoint A = !a b. a IN A /\ b IN A /\ (a <> b) ==> DISJOINT a b`;
 
@@ -771,5 +748,728 @@ val disjoint_union = store_thm
 val disjoint_sing = store_thm
   ("disjoint_sing", ``!a. disjoint {a}``,
     SET_TAC [disjoint_def]);
+
+val disjoint_image = store_thm (* new *)
+  ("disjoint_image",
+  ``!f. (!i j. i <> j ==> DISJOINT (f i) (f j)) ==> disjoint (IMAGE f UNIV)``,
+    rpt STRIP_TAC
+ >> MATCH_MP_TAC disjointI
+ >> RW_TAC std_ss [IN_IMAGE, IN_UNIV]
+ >> METIS_TAC []);
+
+val disjoint_insert = store_thm (* new *)
+  ("disjoint_insert",
+  ``!e c. disjoint (e INSERT c) ==> disjoint c``,
+    RW_TAC std_ss [disjoint_def]
+ >> FIRST_ASSUM MATCH_MP_TAC
+ >> METIS_TAC [IN_INSERT]);
+
+val disjoint_insert_notin = store_thm (* new *)
+  ("disjoint_insert_notin",
+  ``!e c. disjoint (e INSERT c) /\ e NOTIN c ==> !s. s IN c ==> DISJOINT e s``,
+    RW_TAC std_ss [disjoint_def]
+ >> FIRST_ASSUM MATCH_MP_TAC
+ >> METIS_TAC [IN_INSERT]);
+
+(* ------------------------------------------------------------------------- *)
+(*  Some lemmas needed by CARATHEODORY in measureTheory (author: Chun Tian)  *)
+(* ------------------------------------------------------------------------- *)
+
+val DINTER_IMP_FINITE_INTER = store_thm
+  ("DINTER_IMP_FINITE_INTER",
+  ``!sts f. (!s t. s IN sts /\ t IN sts ==> s INTER t IN sts) /\
+            f IN (UNIV -> sts)
+        ==> !n. 0 < n ==> BIGINTER (IMAGE f (count n)) IN sts``,
+    rpt GEN_TAC
+ >> STRIP_TAC
+ >> Induct_on `n`
+ >> RW_TAC arith_ss []
+ >> fs [IN_FUNSET, IN_UNIV]
+ >> STRIP_ASSUME_TAC (Q.SPEC `n` LESS_0_CASES)
+ >- RW_TAC std_ss [COUNT_SUC, COUNT_ZERO, IMAGE_INSERT, IMAGE_EMPTY,
+                   BIGINTER_INSERT, IMAGE_EMPTY, BIGINTER_EMPTY, INTER_UNIV]
+ >> fs [COUNT_SUC]);
+
+(* Dual lemma of above, not used here *)
+val DUNION_IMP_FINITE_UNION = store_thm
+  ("DUNION_IMP_FINITE_UNION",
+  ``!sts f. (!s t. s IN sts /\ t IN sts ==> s UNION t IN sts) /\
+            f IN (UNIV -> sts) ==>
+      !n. 0 < n ==> BIGUNION (IMAGE f (count n)) IN sts``,
+    rpt GEN_TAC
+ >> STRIP_TAC
+ >> Induct_on `n`
+ >> RW_TAC arith_ss []
+ >> fs [IN_FUNSET, IN_UNIV]
+ >> STRIP_ASSUME_TAC (Q.SPEC `n` LESS_0_CASES)
+ >- RW_TAC std_ss [COUNT_SUC, COUNT_ZERO, IMAGE_INSERT, IMAGE_EMPTY,
+                   BIGUNION_INSERT, IMAGE_EMPTY, BIGUNION_EMPTY, UNION_EMPTY]
+ >> fs [COUNT_SUC]);
+
+val GEN_DIFF_INTER = store_thm
+  ("GEN_DIFF_INTER",
+  ``!sp s t. s SUBSET sp /\ t SUBSET sp ==> (s DIFF t = s INTER (sp DIFF t))``,
+    rpt STRIP_TAC
+ >> ASM_SET_TAC []);
+
+val GEN_COMPL_UNION = store_thm
+  ("GEN_COMPL_UNION",
+  ``!sp s t. s SUBSET sp /\ t SUBSET sp ==>
+             (sp DIFF (s UNION t) = (sp DIFF s) INTER (sp DIFF t))``,
+    rpt STRIP_TAC
+ >> ASM_SET_TAC [])
+
+val GEN_COMPL_INTER = store_thm
+  ("GEN_COMPL_INTER",
+  ``!sp s t. s SUBSET sp /\ t SUBSET sp ==>
+             (sp DIFF (s INTER t) = (sp DIFF s) UNION (sp DIFF t))``,
+    rpt STRIP_TAC
+ >> ASM_SET_TAC [])
+
+val GEN_COMPL_FINITE_UNION = store_thm
+  ("GEN_COMPL_FINITE_UNION",
+  ``!sp f n. 0 < n ==> (sp DIFF BIGUNION (IMAGE f (count n)) =
+                        BIGINTER (IMAGE (\i. sp DIFF f i) (count n)))``,
+    NTAC 2 GEN_TAC
+ >> Induct_on `n`
+ >> RW_TAC arith_ss []
+ >> STRIP_ASSUME_TAC (Q.SPEC `n` LESS_0_CASES)
+ >- RW_TAC std_ss [COUNT_SUC, COUNT_ZERO, IMAGE_INSERT, IMAGE_EMPTY, BIGINTER_SING,
+                   BIGUNION_INSERT, IMAGE_EMPTY, BIGUNION_EMPTY, UNION_EMPTY]
+ >> fs [COUNT_SUC]
+ >> ONCE_REWRITE_TAC [UNION_COMM]
+ >> ASM_REWRITE_TAC [DIFF_UNION]
+ >> REWRITE_TAC [DIFF_INTER]
+ >> Suff `(BIGINTER (IMAGE (\i. sp DIFF f i) (count n)) DIFF f n) SUBSET sp`
+ >- (KILL_TAC >> DISCH_THEN (ASSUME_TAC o (MATCH_MP SUBSET_INTER2)) >> ASM_SET_TAC [])
+ >> MATCH_MP_TAC SUBSET_TRANS
+ >> Q.EXISTS_TAC `BIGINTER (IMAGE (\i. sp DIFF f i) (count n))`
+ >> REWRITE_TAC [DIFF_SUBSET]
+ >> REWRITE_TAC [SUBSET_DEF, IN_BIGINTER_IMAGE, IN_COUNT] >> BETA_TAC
+ >> RW_TAC std_ss [IN_DIFF]
+ >> RES_TAC);
+
+val BIGINTER_PAIR = store_thm
+  ("BIGINTER_PAIR",
+  ``!s t. BIGINTER {s; t} = s INTER t``,
+    RW_TAC std_ss [EXTENSION, IN_BIGINTER, IN_INTER, IN_INSERT, NOT_IN_EMPTY]
+ >> PROVE_TAC []);
+
+val DIFF_INTER_PAIR = store_thm
+  ("DIFF_INTER_PAIR",
+  ``!sp x y. sp DIFF (x INTER y) = (sp DIFF x) UNION (sp DIFF y)``,
+    rpt GEN_TAC
+ >> REWRITE_TAC [REWRITE_RULE [BIGINTER_PAIR] (Q.SPECL [`sp`, `{x; y}`] DIFF_BIGINTER1)]
+ >> REWRITE_TAC [EXTENSION, IN_UNION, IN_BIGUNION_IMAGE]
+ >> BETA_TAC
+ >> GEN_TAC >> EQ_TAC >> rpt STRIP_TAC
+ >| [ fs [IN_INSERT] >> PROVE_TAC [],
+      Q.EXISTS_TAC `x` >> ASM_REWRITE_TAC [IN_INSERT],
+      Q.EXISTS_TAC `y` >> ASM_REWRITE_TAC [IN_INSERT] ]);
+
+val GEN_COMPL_FINITE_INTER = store_thm
+  ("GEN_COMPL_FINITE_INTER",
+  ``!sp f n. 0 < n ==> (sp DIFF BIGINTER (IMAGE f (count n)) =
+                        BIGUNION (IMAGE (\i. sp DIFF f i) (count n)))``,
+    NTAC 2 GEN_TAC
+ >> Induct_on `n`
+ >> RW_TAC arith_ss []
+ >> STRIP_ASSUME_TAC (Q.SPEC `n` LESS_0_CASES)
+ >- RW_TAC std_ss [COUNT_SUC, COUNT_ZERO, IMAGE_INSERT, IMAGE_EMPTY, BIGINTER_SING,
+                   BIGUNION_INSERT, IMAGE_EMPTY, BIGUNION_EMPTY, UNION_EMPTY]
+ >> fs [COUNT_SUC]
+ >> ASM_REWRITE_TAC [DIFF_INTER_PAIR]);
+
+(* This proof is provided by Thomas Tuerk, needed by SETS_TO_DISJOINT_SETS *)
+val BIGUNION_IMAGE_COUNT_IMP_UNIV = store_thm
+  ("BIGUNION_IMAGE_COUNT_IMP_UNIV",
+  ``!f g. (!n. BIGUNION (IMAGE g (count n)) = BIGUNION (IMAGE f (count n))) ==>
+          (BIGUNION (IMAGE f UNIV) = BIGUNION (IMAGE g UNIV))``,
+ (* proof *)
+   `!f g. (!n. BIGUNION (IMAGE g (count n)) = BIGUNION (IMAGE f (count n))) ==>
+          (BIGUNION (IMAGE f UNIV) SUBSET BIGUNION (IMAGE g UNIV))`
+       suffices_by PROVE_TAC [SUBSET_ANTISYM]
+ >> REWRITE_TAC [SUBSET_DEF]
+ >> REPEAT STRIP_TAC
+ >> rename1 `e IN BIGUNION _`
+ >> Know `?n. e IN BIGUNION (IMAGE f (count n))`
+ >- (FULL_SIMP_TAC std_ss [IN_BIGUNION, IN_IMAGE, PULL_EXISTS, IN_COUNT] \\
+     rename1 `e IN f n'` \\
+     Q.EXISTS_TAC `SUC n'` \\
+     Q.EXISTS_TAC `n'` \\
+     ASM_SIMP_TAC arith_ss [])
+ >> STRIP_TAC
+ >> `e IN BIGUNION (IMAGE g (count n))` by PROVE_TAC []
+ >> FULL_SIMP_TAC std_ss [IN_BIGUNION, IN_IMAGE, PULL_EXISTS, IN_UNIV]
+ >> METIS_TAC []);
+
+val BIGUNION_OVER_INTER_L = store_thm
+  ("BIGUNION_OVER_INTER_L",
+  ``!f d. BIGUNION (IMAGE f univ(:num)) INTER d =
+          BIGUNION (IMAGE (\i. f i INTER d) univ(:num))``,
+    rpt GEN_TAC
+ >> REWRITE_TAC [EXTENSION]
+ >> GEN_TAC >> EQ_TAC
+ >| [ (* goal 1 (of 2) *)
+      RW_TAC std_ss [IN_BIGUNION, IN_INTER, IN_IMAGE] \\
+      `x IN (f x' INTER d)` by PROVE_TAC [IN_INTER] \\
+      Q.EXISTS_TAC `f x' INTER d` >> art [] \\
+      Q.EXISTS_TAC `x'` >> art [],
+      (* goal 2 (of 2) *)
+      RW_TAC std_ss [IN_BIGUNION, IN_INTER, IN_IMAGE] >|
+      [ fs [IN_INTER] >> Q.EXISTS_TAC `f i` >> ASM_REWRITE_TAC [] \\
+        Q.EXISTS_TAC `i` >> REWRITE_TAC [],
+        PROVE_TAC [IN_INTER] ] ]);
+
+val BIGUNION_OVER_INTER_R = store_thm
+  ("BIGUNION_OVER_INTER_R",
+  ``!f d. d INTER BIGUNION (IMAGE f univ(:num)) =
+          BIGUNION (IMAGE (\i. d INTER f i) univ(:num))``,
+    rpt GEN_TAC
+ >> REWRITE_TAC [EXTENSION]
+ >> GEN_TAC >> EQ_TAC
+ >| [ (* goal 1 (of 2) *)
+      RW_TAC std_ss [IN_BIGUNION, IN_INTER, IN_IMAGE, IN_UNIV] \\
+      `x IN (d INTER f x')` by PROVE_TAC [IN_INTER] \\
+      Q.EXISTS_TAC `d INTER f x'` >> art [] \\
+      Q.EXISTS_TAC `x'` >> art [],
+      (* goal 2 (of 2) *)
+      RW_TAC std_ss [IN_BIGUNION, IN_INTER, IN_IMAGE, IN_UNIV] >|
+      [ fs [IN_INTER] >> Q.EXISTS_TAC `f i` >> ASM_REWRITE_TAC [] \\
+        Q.EXISTS_TAC `i` >> REWRITE_TAC [],
+        PROVE_TAC [IN_INTER] ] ]);
+
+val BIGUNION_OVER_DIFF = store_thm
+  ("BIGUNION_OVER_DIFF",
+  ``!f d. BIGUNION (IMAGE f univ(:num)) DIFF d =
+          BIGUNION (IMAGE (\i. f i DIFF d) univ(:num))``,
+    rpt GEN_TAC
+ >> REWRITE_TAC [EXTENSION]
+ >> GEN_TAC >> EQ_TAC
+ >| [ (* goal 1 (of 2) *)
+      RW_TAC std_ss [IN_BIGUNION, IN_DIFF, IN_IMAGE, IN_UNIV] \\
+      `x IN (f x' DIFF d)` by PROVE_TAC [IN_DIFF] \\
+      Q.EXISTS_TAC `f x' DIFF d` >> art [] \\
+      Q.EXISTS_TAC `x'` >> art [],
+      (* goal 2 (of 2) *)
+      RW_TAC std_ss [IN_BIGUNION, IN_DIFF, IN_IMAGE, IN_UNIV] >|
+      [ fs [IN_DIFF] >> Q.EXISTS_TAC `f i` >> art [] \\
+        Q.EXISTS_TAC `i` >> REWRITE_TAC [],
+        PROVE_TAC [IN_DIFF] ] ]);
+
+val BIGUNION_IMAGE_OVER_INTER_L = store_thm
+  ("BIGUNION_IMAGE_OVER_INTER_L",
+  ``!f n d. BIGUNION (IMAGE f (count n)) INTER d =
+            BIGUNION (IMAGE (\i. f i INTER d) (count n))``,
+    rpt GEN_TAC
+ >> REWRITE_TAC [EXTENSION]
+ >> GEN_TAC >> EQ_TAC
+ >| [ RW_TAC std_ss [IN_BIGUNION, IN_INTER, IN_IMAGE] \\
+      `x IN (f x' INTER d)` by PROVE_TAC [IN_INTER] \\
+      Q.EXISTS_TAC `f x' INTER d` >> art [] \\
+      Q.EXISTS_TAC `x'` >> art [],
+      RW_TAC std_ss [IN_BIGUNION, IN_INTER, IN_IMAGE] >|
+      [ fs [IN_INTER] >> Q.EXISTS_TAC `f i` >> art [] \\
+        Q.EXISTS_TAC `i` >> art [],
+        PROVE_TAC [IN_INTER] ] ]);
+
+val BIGUNION_IMAGE_OVER_INTER_R = store_thm
+  ("BIGUNION_IMAGE_OVER_INTER_R",
+  ``!f n d. d INTER BIGUNION (IMAGE f (count n)) =
+            BIGUNION (IMAGE (\i. d INTER f i) (count n))``,
+    rpt GEN_TAC
+ >> ONCE_REWRITE_TAC [INTER_COMM]
+ >> REWRITE_TAC [BIGUNION_IMAGE_OVER_INTER_L]);
+
+val BIGINTER_IMAGE_OVER_INTER_L = store_thm
+  ("BIGINTER_IMAGE_OVER_INTER_L",
+  ``!f n d. 0 < n ==>
+           (BIGINTER (IMAGE f (count n)) INTER d =
+            BIGINTER (IMAGE (\i. f i INTER d) (count n)))``,
+    rpt STRIP_TAC
+ >> REWRITE_TAC [EXTENSION]
+ >> GEN_TAC >> EQ_TAC
+ >| [ RW_TAC std_ss [IN_BIGINTER_IMAGE, IN_INTER, IN_COUNT],
+      RW_TAC std_ss [IN_BIGINTER_IMAGE, IN_INTER, IN_COUNT] >> RES_TAC ]);
+
+val BIGINTER_IMAGE_OVER_INTER_R = store_thm
+  ("BIGINTER_IMAGE_OVER_INTER_R",
+  ``!f n d. 0 < n ==>
+           (d INTER BIGINTER (IMAGE f (count n)) =
+            BIGINTER (IMAGE (\i. d INTER f i) (count n)))``,
+    rpt STRIP_TAC
+ >> ONCE_REWRITE_TAC [INTER_COMM]
+ >> MATCH_MP_TAC BIGINTER_IMAGE_OVER_INTER_L >> art []);
+
+(* any finite set can be decomposed into a finite sequence of sets *)
+val finite_decomposition_simple = store_thm (* new *)
+  ("finite_decomposition_simple",
+  ``!c. FINITE c ==> ?f n. (!x. x < n ==> f x IN c) /\ (c = IMAGE f (count n))``,
+    GEN_TAC
+ >> REWRITE_TAC [FINITE_BIJ_COUNT_EQ]
+ >> rpt STRIP_TAC
+ >> rename1 `BIJ f (count n) c`
+ >> Q.EXISTS_TAC `f`
+ >> Q.EXISTS_TAC `n`
+ >> CONJ_TAC >- (rpt STRIP_TAC >> PROVE_TAC [BIJ_DEF, INJ_DEF, IN_COUNT])
+ >> PROVE_TAC [BIJ_IMAGE]);
+
+(* any finite set can be decomposed into a finite (non-repeated) sequence of sets *)
+val finite_decomposition = store_thm (* new *)
+  ("finite_decomposition",
+  ``!c. FINITE c ==>
+        ?f n. (!x. x < n ==> f x IN c) /\ (c = IMAGE f (count n)) /\
+              (!i j. i < n /\ j < n /\ i <> j ==> f i <> f j)``,
+    GEN_TAC
+ >> REWRITE_TAC [FINITE_BIJ_COUNT_EQ]
+ >> rpt STRIP_TAC
+ >> rename1 `BIJ f (count n) c`
+ >> Q.EXISTS_TAC `f`
+ >> Q.EXISTS_TAC `n`
+ >> CONJ_TAC >- (rpt STRIP_TAC >> PROVE_TAC [BIJ_DEF, INJ_DEF, IN_COUNT])
+ >> CONJ_TAC >- PROVE_TAC [BIJ_IMAGE]
+ >> rpt STRIP_TAC
+ >> fs [BIJ_ALT, IN_FUNSET, IN_COUNT]
+ >> METIS_TAC []);
+
+(* any finite disjoint set can be decomposed into a finite pair-wise
+   disjoint sequence of sets *)
+val finite_disjoint_decomposition = store_thm (* new *)
+  ("finite_disjoint_decomposition",
+  ``!c. FINITE c /\ disjoint c ==>
+        ?f n. (!i. i < n ==> f i IN c) /\ (c = IMAGE f (count n)) /\
+              (!i j. i < n /\ j < n /\ i <> j ==> f i <> f j) /\
+              (!i j. i < n /\ j < n /\ i <> j ==> DISJOINT (f i) (f j))``,
+    GEN_TAC
+ >> REWRITE_TAC [FINITE_BIJ_COUNT_EQ]
+ >> rpt STRIP_TAC
+ >> rename1 `BIJ f (count n) c`
+ >> Q.EXISTS_TAC `f`
+ >> Q.EXISTS_TAC `n`
+ >> STRONG_CONJ_TAC
+ >- (rpt STRIP_TAC >> PROVE_TAC [BIJ_DEF, INJ_DEF, IN_COUNT])
+ >> DISCH_TAC
+ >> CONJ_TAC >- PROVE_TAC [BIJ_IMAGE]
+ >> STRONG_CONJ_TAC
+ >- (rpt STRIP_TAC \\
+     fs [BIJ_ALT, IN_FUNSET, IN_COUNT] >> METIS_TAC [])
+ >> rpt STRIP_TAC
+ >> fs [disjoint_def]
+ >> FIRST_X_ASSUM MATCH_MP_TAC
+ >> METIS_TAC []);
+
+val countable_disjoint_decomposition = store_thm (* new *)
+  ("countable_disjoint_decomposition",
+  ``!c. FINITE c /\ disjoint c ==>
+        ?f n. (!i. i < n ==> f i IN c) /\ (!i. n <= i ==> (f i = {})) /\
+              (c = IMAGE f (count n)) /\
+              (BIGUNION c = BIGUNION (IMAGE f univ(:num))) /\
+              (!i j. i < n /\ j < n /\ i <> j ==> f i <> f j) /\
+              (!i j. i < n /\ j < n /\ i <> j ==> DISJOINT (f i) (f j))``,
+    rpt STRIP_TAC
+ >> STRIP_ASSUME_TAC
+        (MATCH_MP finite_disjoint_decomposition
+                  (CONJ (ASSUME ``FINITE (c :'a set set)``)
+                        (ASSUME ``disjoint (c :'a set set)``)))
+ >> Q.EXISTS_TAC `\i. if i < n then f i else {}`
+ >> Q.EXISTS_TAC `n`
+ >> BETA_TAC
+ >> CONJ_TAC >- METIS_TAC []
+ >> CONJ_TAC >- METIS_TAC [NOT_LESS]
+ >> CONJ_TAC
+ >- (art [] >> MATCH_MP_TAC IMAGE_CONG >> RW_TAC std_ss [IN_COUNT])
+ >> Reverse CONJ_TAC >- METIS_TAC []
+ >> art [] >> KILL_TAC
+ >> SIMP_TAC std_ss [Once EXTENSION, IN_BIGUNION_IMAGE, IN_COUNT, IN_UNIV]
+ >> GEN_TAC >> EQ_TAC >> rpt STRIP_TAC
+ >| [ Q.EXISTS_TAC `x'` >> METIS_TAC [],
+      Cases_on `i < n` >- (Q.EXISTS_TAC `i` >> METIS_TAC []) \\
+      fs [NOT_IN_EMPTY] ]);
+
+(* any union of two sets can be decomposed into 3 disjoint unions *)
+val UNION_TO_3_DISJOINT_UNIONS = store_thm (* new *)
+  ("UNION_TO_3_DISJOINT_UNIONS",
+  ``!s t. (s UNION t = (s DIFF t) UNION (s INTER t) UNION (t DIFF s)) /\
+          disjoint {(s DIFF t); (s INTER t); (t DIFF s)}``,
+    NTAC 2 GEN_TAC
+ >> CONJ_TAC >- SET_TAC []
+ >> REWRITE_TAC [disjoint_def, DISJOINT_DEF]
+ >> RW_TAC std_ss [IN_INSERT]
+ >> ASM_SET_TAC []);
+
+val DISJOINT_RESTRICT_L = store_thm
+  ("DISJOINT_RESTRICT_L", ``!s t c. DISJOINT s t ==> DISJOINT (s INTER c) (t INTER c)``,
+    SET_TAC [DISJOINT_DEF]);
+
+val DISJOINT_RESTRICT_R = store_thm
+  ("DISJOINT_RESTRICT_R", ``!s t c. DISJOINT s t ==> DISJOINT (c INTER s) (c INTER t)``,
+    SET_TAC [DISJOINT_DEF]);
+
+val SUBSET_RESTRICT_L = store_thm
+  ("SUBSET_RESTRICT_L", ``!r s t. s SUBSET t ==> (s INTER r) SUBSET (t INTER r)``,
+    SET_TAC []);
+
+val SUBSET_RESTRICT_R = store_thm
+  ("SUBSET_RESTRICT_R", ``!r s t. s SUBSET t ==> (r INTER s) SUBSET (r INTER t)``,
+    SET_TAC []);
+
+val SUBSET_RESTRICT_DIFF = store_thm
+  ("SUBSET_RESTRICT_DIFF", ``!r s t. s SUBSET t ==> (r DIFF t) SUBSET (r DIFF s)``,
+    SET_TAC []);
+
+val SUBSET_INTER_SUBSET_L = store_thm
+  ("SUBSET_INTER_SUBSET_L", ``!r s t. s SUBSET t ==> (s INTER r) SUBSET t``,
+    SET_TAC []);
+
+val SUBSET_INTER_SUBSET_R = store_thm
+  ("SUBSET_INTER_SUBSET_R", ``!r s t. s SUBSET t ==> (r INTER s) SUBSET t``,
+    SET_TAC []);
+
+val SUBSET_MONO_DIFF = store_thm
+  ("SUBSET_MONO_DIFF", ``!r s t. s SUBSET t ==> (s DIFF r) SUBSET (t DIFF r)``,
+    SET_TAC []);
+
+val SUBSET_DIFF_SUBSET = store_thm
+  ("SUBSET_DIFF_SUBSET", ``!r s t. s SUBSET t ==> (s DIFF r) SUBSET t``,
+    SET_TAC []);
+
+val BIGUNION_IMAGE_BIGUNION_IMAGE_UNIV = store_thm
+  ("BIGUNION_IMAGE_BIGUNION_IMAGE_UNIV",
+  ``!f. BIGUNION (IMAGE (\n. BIGUNION (IMAGE (f n) univ(:num))) univ(:num)) =
+        BIGUNION (IMAGE (UNCURRY f) univ(:num # num))``,
+    GEN_TAC
+ >> RW_TAC std_ss [EXTENSION, IN_BIGUNION_IMAGE, IN_UNIV, IN_CROSS, UNCURRY]
+ >> EQ_TAC >> STRIP_TAC
+ >- (Q.EXISTS_TAC `(n, x')` >> art [FST, SND])
+ >> Q.EXISTS_TAC `FST x'`
+ >> Q.EXISTS_TAC `SND x'` >> art []);
+
+val BIGUNION_IMAGE_UNIV_CROSS_UNIV = store_thm
+  ("BIGUNION_IMAGE_UNIV_CROSS_UNIV",
+  ``!f (h :num -> num # num). BIJ h UNIV (UNIV CROSS UNIV) ==>
+       (BIGUNION (IMAGE (UNCURRY f) univ(:num # num)) =
+        BIGUNION (IMAGE (UNCURRY f o h) univ(:num)))``,
+    rpt STRIP_TAC
+ >> RW_TAC std_ss [EXTENSION, IN_BIGUNION_IMAGE, IN_UNIV, IN_CROSS, UNCURRY, o_DEF]
+ >> fs [BIJ_ALT, IN_FUNSET, IN_UNIV]
+ >> EQ_TAC >> STRIP_TAC
+ >- (Q.PAT_X_ASSUM `!y. ?!x. y = h x` (MP_TAC o (Q.SPEC `x'`)) >> METIS_TAC [])
+ >> Q.EXISTS_TAC `h x'` >> art []);
+
+
+(* ------------------------------------------------------------------------- *)
+(*  Three series of lemmas on bigunion-equivalent sequences of sets          *)
+(* ------------------------------------------------------------------------- *)
+
+(* 1. for any sequence of sets, there is an increasing sequence of the same bigunion. *)
+val SETS_TO_INCREASING_SETS = store_thm
+  ("SETS_TO_INCREASING_SETS",
+  ``!f :num->'a set.
+       ?g. (g 0 = f 0) /\ (!n. g n = BIGUNION (IMAGE f (count (SUC n)))) /\
+           (!n. g n SUBSET g (SUC n)) /\
+           (BIGUNION (IMAGE f UNIV) = BIGUNION (IMAGE g UNIV))``,
+    rpt STRIP_TAC
+ >> Q.EXISTS_TAC `\n. BIGUNION (IMAGE f (count (SUC n)))`
+ >> BETA_TAC
+ >> RW_TAC bool_ss []
+ >| [ (* goal 1 (of 3) *)
+      REWRITE_TAC [COUNT_SUC, COUNT_ZERO, IMAGE_SING, BIGUNION_SING],
+      (* goal 2 (of 3) *)
+     `count (SUC (SUC n)) = (SUC n) INSERT (count (SUC n))`
+          by PROVE_TAC [COUNT_SUC] >> POP_ORW \\
+      REWRITE_TAC [IMAGE_INSERT, BIGUNION_INSERT] \\
+      REWRITE_TAC [SUBSET_UNION],
+      (* goal 3 (of 3) *)
+      MATCH_MP_TAC BIGUNION_IMAGE_COUNT_IMP_UNIV \\
+      Induct_on `n` >- REWRITE_TAC [COUNT_ZERO, IMAGE_EMPTY, BIGUNION_EMPTY] \\
+     `count (SUC n) = n INSERT (count n)` by PROVE_TAC [COUNT_SUC] \\
+      POP_ORW >> REWRITE_TAC [IMAGE_INSERT, BIGUNION_INSERT] \\
+      POP_ASSUM (REWRITE_TAC o wrap) \\
+      BETA_TAC \\
+      Cases_on `n = 0` >> fs [COUNT_SUC, COUNT_ZERO, IMAGE_SING, BIGUNION_SING] \\
+      REWRITE_TAC [GSYM UNION_ASSOC, UNION_IDEMPOT] ]);
+
+(* another version with `g 0 = {}` *)
+val SETS_TO_INCREASING_SETS' = store_thm
+  ("SETS_TO_INCREASING_SETS'",
+  ``!f :num -> 'a set.
+       ?g. (g 0 = {}) /\ (!n. g n = BIGUNION (IMAGE f (count n))) /\
+           (!n. g n SUBSET g (SUC n)) /\
+           (BIGUNION (IMAGE f UNIV) = BIGUNION (IMAGE g UNIV))``,
+    rpt STRIP_TAC
+ >> Q.EXISTS_TAC `\n. BIGUNION (IMAGE f (count n))`
+ >> BETA_TAC
+ >> RW_TAC bool_ss []
+ >| [ (* goal 1 (of 3) *)
+      REWRITE_TAC [COUNT_ZERO, IMAGE_EMPTY, BIGUNION_EMPTY],
+      (* goal 2 (of 3) *)
+     `count (SUC n) = n INSERT (count n)` by PROVE_TAC [COUNT_SUC] \\
+      POP_ORW >> REWRITE_TAC [IMAGE_INSERT, BIGUNION_INSERT] \\
+      REWRITE_TAC [SUBSET_UNION],
+      (* goal 3 (of 3) *)
+      REWRITE_TAC [EXTENSION] \\
+      GEN_TAC >> SIMP_TAC std_ss [IN_BIGUNION_IMAGE, IN_UNIV, IN_COUNT] \\
+      EQ_TAC >> RW_TAC std_ss [] >|
+      [ Q.EXISTS_TAC `SUC x'` \\
+        Q.EXISTS_TAC `x'` >> ASM_SIMP_TAC arith_ss [],
+        Q.EXISTS_TAC `x'` >> art [] ] ]);
+
+(* 2. (hard) for any sequence of sets in a space, there is a disjoint family with
+      the same bigunion. This lemma is needed by DYNKIN_LEMMA *)
+val SETS_TO_DISJOINT_SETS = store_thm
+  ("SETS_TO_DISJOINT_SETS",
+  ``!sp sts f. (!s. s IN sts ==> s SUBSET sp) /\ (!n. f n IN sts) ==>
+       ?g. (g 0 = f 0) /\
+           (!n. 0 < n ==> (g n = f n INTER (BIGINTER (IMAGE (\i. sp DIFF f i) (count n))))) /\
+           (!i j :num. i <> j ==> DISJOINT (g i) (g j)) /\
+           (BIGUNION (IMAGE f UNIV) = BIGUNION (IMAGE g UNIV))``,
+    rpt STRIP_TAC
+ >> Q.EXISTS_TAC `\n. if n = 0:num then f n
+                      else f n INTER (BIGINTER (IMAGE (\i. sp DIFF f i) (count n)))`
+ >> BETA_TAC >> SIMP_TAC arith_ss []
+ >> CONJ_TAC >> RW_TAC arith_ss []
+ >| [ (* goal 1 (of 4)
+        `DISJOINT (f 0) (f j INTER BIGINTER (IMAGE (\i. sp DIFF f i) (count j)))` *)
+      `0 IN (count j)` by PROVE_TAC [NOT_ZERO_LT_ZERO, IN_COUNT] \\
+      POP_ASSUM (MP_TAC o SYM o (MATCH_MP INSERT_DELETE)) \\
+      DISCH_THEN (ONCE_REWRITE_TAC o wrap) \\
+      REWRITE_TAC [IMAGE_INSERT, BIGINTER_INSERT] >> BETA_TAC \\
+      REWRITE_TAC [INTER_ASSOC] \\
+      `f j INTER (sp DIFF f 0) = (sp DIFF f 0) INTER f j` by PROVE_TAC [INTER_COMM] \\
+      POP_ASSUM (ONCE_REWRITE_TAC o wrap) \\
+      REWRITE_TAC [DIFF_INTER, DISJOINT_DIFF],
+      (* goal 2 (of 4),
+        `DISJOINT (f i INTER BIGINTER (IMAGE (\i. sp DIFF f i) (count i))) (f 0)` *)
+     `0 IN (count i)` by PROVE_TAC [NOT_ZERO_LT_ZERO, IN_COUNT] \\
+      POP_ASSUM (MP_TAC o SYM o (MATCH_MP INSERT_DELETE)) \\
+      DISCH_THEN (ONCE_REWRITE_TAC o wrap) \\
+      REWRITE_TAC [IMAGE_INSERT, BIGINTER_INSERT] >> BETA_TAC \\
+      REWRITE_TAC [INTER_ASSOC] \\
+     `f i INTER (sp DIFF f 0) = (sp DIFF f 0) INTER f i` by PROVE_TAC [INTER_COMM] \\
+      POP_ASSUM (ONCE_REWRITE_TAC o wrap) \\
+      REWRITE_TAC [DIFF_INTER, DISJOINT_DIFF],
+      (* goal 3 (of 4),
+        `DISJOINT (f i INTER BIGINTER (IMAGE (\i. sp DIFF f i) (count i)))
+                  (f j INTER BIGINTER (IMAGE (\i. sp DIFF f i) (count j)))` *)
+      STRIP_ASSUME_TAC (Q.SPECL [`i`, `j`] LESS_LESS_CASES) >| (* 2 subgoals *)
+      [ (* goal 3.1 (of 2) *)
+        ONCE_REWRITE_TAC [DISJOINT_SYM] \\
+        MATCH_MP_TAC DISJOINT_SUBSET \\
+        Q.EXISTS_TAC `f i` >> REWRITE_TAC [INTER_SUBSET] \\
+       `i IN (count j)` by PROVE_TAC [IN_COUNT] \\
+        POP_ASSUM (MP_TAC o SYM o (MATCH_MP INSERT_DELETE)) \\
+        DISCH_THEN (ONCE_REWRITE_TAC o wrap) \\
+        REWRITE_TAC [IMAGE_INSERT, BIGINTER_INSERT] >> BETA_TAC \\
+        REWRITE_TAC [INTER_ASSOC] \\
+       `f j INTER (sp DIFF f i) = (sp DIFF f i) INTER f j` by PROVE_TAC [INTER_COMM] \\
+        POP_ASSUM (ONCE_REWRITE_TAC o wrap) \\
+        REWRITE_TAC [DIFF_INTER, DISJOINT_DIFF],
+        (* goal 3.2 (of 2) *)
+        MATCH_MP_TAC DISJOINT_SUBSET \\
+        Q.EXISTS_TAC `f j` >> REWRITE_TAC [INTER_SUBSET] \\
+       `j IN (count i)` by PROVE_TAC [IN_COUNT] \\
+        POP_ASSUM (MP_TAC o SYM o (MATCH_MP INSERT_DELETE)) \\
+        DISCH_THEN (ONCE_REWRITE_TAC o wrap) \\
+        REWRITE_TAC [IMAGE_INSERT, BIGINTER_INSERT] >> BETA_TAC \\
+        REWRITE_TAC [INTER_ASSOC] \\
+       `f i INTER (sp DIFF f j) = (sp DIFF f j) INTER f i` by PROVE_TAC [INTER_COMM] \\
+        POP_ASSUM (ONCE_REWRITE_TAC o wrap) \\
+        REWRITE_TAC [DIFF_INTER, DISJOINT_DIFF] ],
+      (* goal 4 (of 4) *)
+      MATCH_MP_TAC BIGUNION_IMAGE_COUNT_IMP_UNIV \\
+      Induct_on `n` >- REWRITE_TAC [COUNT_ZERO, IMAGE_EMPTY, BIGUNION_EMPTY] \\
+      REWRITE_TAC [COUNT_SUC, IMAGE_INSERT, BIGUNION_INSERT] \\
+      POP_ASSUM (REWRITE_TAC o wrap) >> BETA_TAC \\
+      Cases_on `n = 0` >> fs [] (* now ``n <> 0`` *) \\
+      REWRITE_TAC [Once UNION_COMM, INTER_OVER_UNION] \\
+      GEN_REWRITE_TAC (RAND_CONV o ONCE_DEPTH_CONV) empty_rewrites [UNION_COMM] \\
+      Suff `BIGUNION (IMAGE f (count n)) UNION (BIGINTER (IMAGE (\i. sp DIFF f i) (count n))) = sp`
+      >- (DISCH_THEN (REWRITE_TAC o wrap) \\
+          REWRITE_TAC [INTER_SUBSET_EQN, UNION_SUBSET] \\
+          Reverse CONJ_TAC >- PROVE_TAC [] \\
+          REWRITE_TAC [BIGUNION_SUBSET, IN_IMAGE] >> PROVE_TAC []) \\
+      (* BIGUNION (IMAGE f (count n)) UNION BIGINTER (IMAGE (\i. sp DIFF f i) (count n)) = sp *)
+     `0 < n` by PROVE_TAC [NOT_ZERO_LT_ZERO] \\
+      POP_ASSUM (REWRITE_TAC o wrap o GSYM o (MATCH_MP GEN_COMPL_FINITE_UNION)) \\
+      Suff `BIGUNION (IMAGE f (count n)) SUBSET sp` >- ASM_SET_TAC [] \\
+      REWRITE_TAC [BIGUNION_SUBSET, IN_IMAGE] >> PROVE_TAC [] ]);
+
+(* A specific version without sts and sp *)
+val SETS_TO_DISJOINT_SETS' = store_thm
+  ("SETS_TO_DISJOINT_SETS'",
+  ``!f. ?g. (g 0 = f 0) /\
+            (!n. 0 < n ==> (g n = f n INTER (BIGINTER (IMAGE (COMPL o f) (count n))))) /\
+            (!i j :num. i <> j ==> DISJOINT (g i) (g j)) /\
+            (BIGUNION (IMAGE f UNIV) = BIGUNION (IMAGE g UNIV))``,
+    GEN_TAC
+ >> STRIP_ASSUME_TAC (Q.SPECL [`UNIV`, `UNIV`, `f`] SETS_TO_DISJOINT_SETS)
+ >> fs [SUBSET_UNIV, o_DEF, COMPL_DEF]
+ >> Q.EXISTS_TAC `g` >> art []);
+
+(* 3. (hard) for any sequence of (straightly) increasing sets, there is a disjoint
+      family with the same bigunion. *)
+val INCREASING_TO_DISJOINT_SETS = store_thm
+  ("INCREASING_TO_DISJOINT_SETS",
+  ``!f :num -> 'a set. (!n. f n SUBSET f (SUC n)) ==>
+       ?g. (g 0 = f 0) /\ (!n. 0 < n ==> (g n = f n DIFF f (PRE n))) /\
+           (!i j :num. i <> j ==> DISJOINT (g i) (g j)) /\
+           (BIGUNION (IMAGE f UNIV) = BIGUNION (IMAGE g UNIV))``,
+    rpt STRIP_TAC
+ >> Q.EXISTS_TAC `\n. if n = (0 :num) then f n else f n DIFF f (PRE n)`
+ >> BETA_TAC
+ (* preliminaries *)
+ >> Know `!n. 0 < n ==> f 0 SUBSET (f n)`
+ >- (Induct_on `n` >- RW_TAC arith_ss [] \\
+     RW_TAC arith_ss [] \\
+     Cases_on `n = 0` >- art [] \\
+     IMP_RES_TAC NOT_ZERO_LT_ZERO >> RES_TAC \\
+     MATCH_MP_TAC SUBSET_TRANS >> Q.EXISTS_TAC `f n` >> art [])
+ >> DISCH_TAC
+ >> Know `!n. 0 < n ==> f 0 SUBSET (f (PRE n))`
+ >- (Induct_on `n` >- RW_TAC arith_ss [] \\
+     RW_TAC arith_ss [] \\
+     Cases_on `n = 0` >- art [SUBSET_REFL] \\
+     IMP_RES_TAC NOT_ZERO_LT_ZERO >> RES_TAC)
+ >> DISCH_TAC
+ >> Know `!i j. i < j ==> f (SUC i) SUBSET (f j)`
+ >- (GEN_TAC >> Induct_on `j` >- RW_TAC arith_ss [] \\
+     STRIP_TAC \\
+     fs [GSYM LESS_EQ_IFF_LESS_SUC, LESS_OR_EQ] \\
+     MATCH_MP_TAC SUBSET_TRANS >> Q.EXISTS_TAC `f j` \\
+     CONJ_TAC >- RES_TAC >> art [])
+ >> DISCH_TAC
+ >> Know `!n. 0 < n ==> f (PRE n) SUBSET f n`
+ >- (rpt STRIP_TAC \\
+     Q.PAT_X_ASSUM `!n. f n SUBSET f (SUC n)` (STRIP_ASSUME_TAC o (Q.SPEC `PRE n`)) \\
+     PROVE_TAC [SUC_PRE])
+ >> DISCH_TAC
+ >> Know `!i j. i < j ==> f i SUBSET f (PRE j)`
+ >- (GEN_TAC >> Induct_on `j` >- RW_TAC arith_ss [] \\
+     STRIP_TAC \\
+     fs [GSYM LESS_EQ_IFF_LESS_SUC, LESS_OR_EQ] \\
+     MATCH_MP_TAC SUBSET_TRANS >> Q.EXISTS_TAC `f (PRE j)` \\
+     CONJ_TAC >- RES_TAC \\
+     Cases_on `j = 0` >- (RW_TAC arith_ss [SUBSET_REFL]) \\
+     IMP_RES_TAC NOT_ZERO_LT_ZERO >> RES_TAC)
+ >> DISCH_TAC
+ >> RW_TAC arith_ss []
+ >| [ (* goal 1 (of 4): DISJOINT (f 0) (f (SUC j) DIFF f j) *)
+      MATCH_MP_TAC SUBSET_DIFF_DISJOINT \\
+      Q.EXISTS_TAC `f j` \\
+      IMP_RES_TAC NOT_ZERO_LT_ZERO \\
+     `f j DIFF (f j DIFF f (PRE j)) = f (PRE j)`
+          by PROVE_TAC [DIFF_DIFF_SUBSET] >> POP_ORW >> RES_TAC,
+      (* goal 2 (of 4): DISJOINT (f (SUC i) DIFF f i) (f 0) *)
+      ONCE_REWRITE_TAC [DISJOINT_SYM] \\
+      MATCH_MP_TAC SUBSET_DIFF_DISJOINT \\
+      Q.EXISTS_TAC `f i` \\
+      IMP_RES_TAC NOT_ZERO_LT_ZERO \\
+     `f i DIFF (f i DIFF f (PRE i)) = f (PRE i)`
+          by PROVE_TAC [DIFF_DIFF_SUBSET] >> POP_ORW \\
+      IMP_RES_TAC NOT_ZERO_LT_ZERO >> RES_TAC,
+      (* goal 3 (of 4): DISJOINT (f (SUC i) DIFF f i) (f (SUC j) DIFF f j) *)
+      STRIP_ASSUME_TAC (Q.SPECL [`i`, `j`] LESS_LESS_CASES) >| (* 2 subgoals *)
+      [ (* goal 3.1 (of 2) *)
+        ONCE_REWRITE_TAC [DISJOINT_SYM] \\
+        MATCH_MP_TAC DISJOINT_SUBSET \\
+        Q.EXISTS_TAC `f i` >> REWRITE_TAC [DIFF_SUBSET] \\
+        ONCE_REWRITE_TAC [DISJOINT_SYM] \\
+        MATCH_MP_TAC SUBSET_DIFF_DISJOINT \\
+        Q.EXISTS_TAC `f j` \\
+        IMP_RES_TAC NOT_ZERO_LT_ZERO \\
+       `f j DIFF (f j DIFF f (PRE j)) = f (PRE j)`
+          by PROVE_TAC [DIFF_DIFF_SUBSET] >> POP_ORW >> RES_TAC,
+        (* goal 3.2 (of 2) *)
+        MATCH_MP_TAC DISJOINT_SUBSET \\
+        Q.EXISTS_TAC `f j` >> REWRITE_TAC [DIFF_SUBSET] \\
+        ONCE_REWRITE_TAC [DISJOINT_SYM] \\
+        MATCH_MP_TAC SUBSET_DIFF_DISJOINT \\
+        Q.EXISTS_TAC `f i` \\
+        IMP_RES_TAC NOT_ZERO_LT_ZERO \\
+       `f i DIFF (f i DIFF f (PRE i)) = f (PRE i)`
+          by PROVE_TAC [DIFF_DIFF_SUBSET] >> POP_ORW >> RES_TAC ],
+      (* goal 4 (of 4): BIGUNION (IMAGE f univ(:num)) = ... *)
+      MATCH_MP_TAC BIGUNION_IMAGE_COUNT_IMP_UNIV \\
+      Induct_on `n` >- REWRITE_TAC [COUNT_ZERO, IMAGE_EMPTY, BIGUNION_EMPTY] \\
+      REWRITE_TAC [COUNT_SUC, IMAGE_INSERT, BIGUNION_INSERT] \\
+      POP_ASSUM (REWRITE_TAC o wrap) >> BETA_TAC \\
+      Cases_on `n = 0` >> fs [] (* now ``n <> 0`` *) \\
+      RW_TAC arith_ss [EXTENSION, IN_UNION, IN_BIGUNION_IMAGE, IN_COUNT, IN_DIFF] \\
+      EQ_TAC >> rpt STRIP_TAC >| (* 4 subgoals *)
+      [ DISJ1_TAC >> art [],
+        DISJ2_TAC >> Q.EXISTS_TAC `x'` >> art [],
+        Cases_on `x IN f (PRE n)` >- (DISJ2_TAC >> Q.EXISTS_TAC `PRE n` \\
+                                      ASM_SIMP_TAC arith_ss []) \\
+        DISJ1_TAC >> art [],
+        DISJ2_TAC >> Q.EXISTS_TAC `x'` >> art [] ] ]);
+
+(* Surprisingly, this variant of INCREASING_TO_DISJOINT_SETS cannot be
+   easily proved without using the non-trivial SETS_TO_DISJOINT_SETS *)
+val INCREASING_TO_DISJOINT_SETS' = store_thm
+  ("INCREASING_TO_DISJOINT_SETS'",
+  ``!f :num -> 'a set. (f 0 = {}) /\ (!n. f n SUBSET f (SUC n)) ==>
+       ?g. (!n. g n = f (SUC n) DIFF f n) /\
+           (!i j :num. i <> j ==> DISJOINT (g i) (g j)) /\
+           (BIGUNION (IMAGE f UNIV) = BIGUNION (IMAGE g UNIV))``,
+    rpt STRIP_TAC
+ >> Q.EXISTS_TAC `\n. f (SUC n) DIFF f n`
+ >> BETA_TAC
+ (* preliminaries *)
+ >> Know `!i j. i < j ==> f i SUBSET f j`
+ >- (GEN_TAC >> Induct_on `j` >- RW_TAC arith_ss [] \\
+     STRIP_TAC \\
+     MATCH_MP_TAC SUBSET_TRANS >> Q.EXISTS_TAC `f j` >> art [] \\
+     fs [GSYM LESS_EQ_IFF_LESS_SUC, LESS_OR_EQ])
+ >> DISCH_TAC
+ >> Know `!i j. i < j ==> f (SUC i) SUBSET f j`
+ >- (GEN_TAC >> Induct_on `j` >- RW_TAC arith_ss [] \\
+     STRIP_TAC \\
+     Cases_on `i = j` >- PROVE_TAC [SUBSET_REFL] \\
+     MATCH_MP_TAC SUBSET_TRANS >> Q.EXISTS_TAC `f j` >> art [] \\
+     fs [GSYM LESS_EQ_IFF_LESS_SUC, LESS_OR_EQ])
+ >> DISCH_TAC
+ >> RW_TAC arith_ss [] (* 2 subgoals *)
+ >| [ (* goal 1 (of 2): DISJOINT (f (SUC i) DIFF f i) (f (SUC j) DIFF f j) *)
+      STRIP_ASSUME_TAC (Q.SPECL [`i`, `j`] LESS_LESS_CASES) >| (* 2 subgoals *)
+      [ (* goal 1.1 (of 2) *)
+        ONCE_REWRITE_TAC [DISJOINT_SYM] \\
+        MATCH_MP_TAC DISJOINT_SUBSET \\
+        Q.EXISTS_TAC `f (SUC i)` >> REWRITE_TAC [DIFF_SUBSET] \\
+        ONCE_REWRITE_TAC [DISJOINT_SYM] \\
+        MATCH_MP_TAC SUBSET_DIFF_DISJOINT \\
+        Q.EXISTS_TAC `f (SUC j)` \\
+        `f (SUC j) DIFF (f (SUC j) DIFF f j) = f j`
+          by PROVE_TAC [DIFF_DIFF_SUBSET] >> POP_ORW >> RES_TAC,
+        (* goal 1.2 (of 2) *)
+        MATCH_MP_TAC DISJOINT_SUBSET \\
+        Q.EXISTS_TAC `f (SUC j)` >> REWRITE_TAC [DIFF_SUBSET] \\
+        ONCE_REWRITE_TAC [DISJOINT_SYM] \\
+        MATCH_MP_TAC SUBSET_DIFF_DISJOINT \\
+        Q.EXISTS_TAC `f (SUC i)` \\
+       `f (SUC i) DIFF (f (SUC i) DIFF f i) = f i`
+          by PROVE_TAC [DIFF_DIFF_SUBSET] >> POP_ORW >> RES_TAC ],
+      (* goal 2 (of 2): BIGUNION (IMAGE f univ(:num)) = ... *)
+      STRIP_ASSUME_TAC (Q.SPEC `f` SETS_TO_DISJOINT_SETS') >> art [] \\
+      RW_TAC std_ss [EXTENSION, IN_BIGUNION_IMAGE, IN_UNIV, IN_DIFF] \\
+      EQ_TAC >> rpt STRIP_TAC >| (* 2 subgoals *)
+      [ (* goal 2.1 (of 2) *)
+        Cases_on `x' = 0` >- PROVE_TAC [NOT_IN_EMPTY] \\
+        IMP_RES_TAC NOT_ZERO_LT_ZERO \\
+        Q.EXISTS_TAC `PRE x'` \\
+       `SUC (PRE x') = x'` by PROVE_TAC [SUC_PRE] >> POP_ORW \\
+        Q.PAT_X_ASSUM `x IN g x'` MP_TAC \\
+        Q.PAT_X_ASSUM `!n. 0 < n ==> X`
+            (fn th => REWRITE_TAC [MATCH_MP th (ASSUME ``0:num < x'``)]) \\
+        RW_TAC std_ss [IN_INTER, IN_BIGINTER_IMAGE, IN_COUNT, o_DEF, IN_COMPL] \\
+        FIRST_X_ASSUM MATCH_MP_TAC >> RW_TAC arith_ss [],
+        (* goal 2.2 (of 2) *)
+        Q.EXISTS_TAC `SUC n` \\
+       `0 < SUC n` by REWRITE_TAC [prim_recTheory.LESS_0] \\
+        Q.PAT_X_ASSUM `!n. 0 < n ==> X`
+            (fn th => REWRITE_TAC [MATCH_MP th (ASSUME ``0:num < SUC n``)]) \\
+        RW_TAC std_ss [IN_INTER, IN_BIGINTER_IMAGE, IN_COUNT, o_DEF, IN_COMPL] \\
+        fs [GSYM LESS_EQ_IFF_LESS_SUC, LESS_OR_EQ] \\
+        CCONTR_TAC >> fs [] \\
+       `x IN f n` by PROVE_TAC [SUBSET_DEF] ] ]);
 
 val _ = export_theory ();
