src/probability/README.md
@@ -1,0 +1,46 @@
+# HOL's Probability Theory
+
+This directory contains HOL4's Measure, Lebesgue integral and
+Probability theories.
+
+## Measure, Integral and Probability Theory defined on extended reals (new)
+
+     extrealScript.sml     * The theory of Extended Real Numbers
+     measureScript.sml     * Measure Theory defined on extended reals
+     borelScript.sml       * Borel sets and Borel measurable functions
+     lebesgueScript.sml    * The theory of Lebesgue Integral
+     martingaleScript.sml  * The theory of martingales based on σ-finite filtered measure space
+     probabilityScript.sml * Probability Theory (toplevel)
+
+## Measure and Probability Theory defined on reals (old)
+
+     obsoleted/old_measureScript.sml
+     obsoleted/old_borelScript.sml
+     obsoleted/old_lebesgueScript.sml
+     obsoleted/old_probabilityScript.sml
+
+(These old scripts are used by `examples/miller` and `examples/diningcryptos`)
+
+## Elementary Topology in Euclidean Space (from hol-light)
+
+     real_topologyScript.sml
+
+## Utilities
+
+     hurdUtils.{sml|sig}   * some useful tools created by Joe Hurd
+     util_probScript.sml   * utility lemmas needed by other scripts
+     iterateScript.sml     * utility theory used by real_topologyScript.sml
+     productScript.sml     * utility theory used by real_topologyScript.sml
+
+## Contributors
+
+- Valentina Bruno (hol-light)
+- Aaron Coble
+- John Harrison (hol-light)
+- Osman Hasan
+- Joe Hurd
+- Marco Maggesi (hol-light)
+- Tarek Mhamdi
+- Muhammad Qasim
+- Sofiene Tahar
+- Chun Tian
